added old file for comparison

armv8_lifter_rework_IL_heavy.v
@@ -10,7 +10,6 @@ Unset Printing All.
 Require Import Picinae_armv8_pcode Picinae_armv8_PIL_notation.
 Import Picinae_armv8_PIL_notation.Notation.
 Require Import List String Ascii NArith Bool.
-Require Import ZArith.
 Import ListNotations.
 Local Open Scope string_scope.
 Local Open Scope N_scope.
@@ -76,7 +75,7 @@ Module Notation.
       if match_all_patterns ns pats then act
       else select_pattern_list ns default cases'
     end.
-  Notation "pats => val" := (pats, val) (at level 201, only parsing).
+  Notation "pats => val" := (pats, val) (at level 201).
   Notation "'match[bits]' n0 , .. , nn 'with' | c0 | .. | cn 'else' d 'end'" := (
      match n0::..[nn].., c0::..[cn].. with ns, cases =>
        ltac:(let r := eval cbn in (select_pattern_list ns d cases) in exact r)
@@ -103,41 +102,16 @@ Notation "'PC'" := (Var R_PC) (in custom PIL at level 65).
     return;
   *)
 
-Definition XtoVar n := 
-  match n with
-  | 0 => Var R_X0
-  | 1 => Var R_X1
-  | 2 => Var R_X2
-  | 3 => Var R_X3
-  | 4 => Var R_X4
-  | 5 => Var R_X5
-  | 6 => Var R_X6
-  | 7 => Var R_X7
-  | 8 => Var R_X8
-  | 9 => Var R_X9
-  | 10 => Var R_X10
-  | 11 => Var R_X11
-  | 12 => Var R_X12
-  | 13 => Var R_X13
-  | 14 => Var R_X14
-  | 15 => Var R_X15
-  | 16 => Var R_X16
-  | 17 => Var R_X17
-  | 18 => Var R_X18
-  | 19 => Var R_X19
-  | 20 => Var R_X20
-  | 21 => Var R_X21
-  | 22 => Var R_X22
-  | 23 => Var R_X23
-  | 24 => Var R_X24
-  | 25 => Var R_X25
-  | 26 => Var R_X26
-  | 27 => Var R_X27
-  | 28 => Var R_X28
-  | 29 => Var R_X29
-  | 30 => Var R_X30
-  | _ => Var R_SP
-  end.
+Definition XtoVar n := let n := <{n#5}> in <{
+  ite (n = (0#5)) {Var R_X0} ( ite (n = (1#5)) {Var R_X1} ( ite (n = (2#5)) {Var R_X2} ( ite (n = (3#5)) {Var R_X3} (
+  ite (n = (4#5)) {Var R_X4} ( ite (n = (5#5)) {Var R_X5} ( ite (n = (6#5)) {Var R_X6} ( ite (n = (7#5)) {Var R_X7} (
+  ite (n = (8#5)) {Var R_X8} ( ite (n = (9#5)) {Var R_X9} ( ite (n = (10#5)) {Var R_X10} ( ite (n = (11#5)) {Var R_X11} (
+  ite (n = (12#5)) {Var R_X12} ( ite (n = (13#5)) {Var R_X13} ( ite (n = (14#5)) {Var R_X14} ( ite (n = (15#5)) {Var R_X15} (
+  ite (n = (16#5)) {Var R_X16} ( ite (n = (17#5)) {Var R_X17} ( ite (n = (18#5)) {Var R_X18} ( ite (n = (19#5)) {Var R_X19} (
+  ite (n = (20#5)) {Var R_X20} ( ite (n = (21#5)) {Var R_X21} ( ite (n = (22#5)) {Var R_X22} ( ite (n = (23#5)) {Var R_X23} (
+  ite (n = (24#5)) {Var R_X24} ( ite (n = (25#5)) {Var R_X25} ( ite (n = (26#5)) {Var R_X26} ( ite (n = (27#5)) {Var R_X27} (
+  ite (n = (28#5)) {Var R_X28} ( ite (n = (29#5)) {Var R_X29} ( ite (n = (30#5)) {Var R_X30} {Var R_SP}))))))))))))))))))))))))))))))
+}>.
 
 Definition arm_varid n :=
   match n with
@@ -169,7 +143,7 @@ Notation "'temp[' n ']'" := (V_TEMP n) (at level 65, no associativity).
 Definition arm_assign_R n val := Move (arm_varid n) val. (*TODO: Need to fix this*)
 Definition arm_assign_flags flags :=
     let '(n, z, c, v) := Unpack_NZCV flags in
-
+    
     (Seq (Move R_NG n) (Seq (Move R_ZR z) (Seq (Move R_CY c) (Move R_OV v)))).
 
 Definition arm64_R n N :=
@@ -264,7 +238,7 @@ Definition ConditionHolds (cond:N) : exp :=
 
 (* Assume LittleE only execution. The documentation for Big Endian
    is a little confusing and sparse (J1-7567). *)
-Definition BigEndian : exp := <{0#1}>.
+Definition BigEndian : exp := <{0#0}>.
 
 (* Configure Atomic extension, for now it seems to be supportable.
    We do not model concurrency so these are just regular operations. *)
@@ -313,12 +287,12 @@ Variant arm_add_sub_imm :=
   | ARM_SUBS_IMM.
 (*Logical (imm), Bitfield*)
 Variant arm_logical_imm :=
-  | ARM_AND_IMM
+  | ARM_AND_IMM 
   | ARM_ANDS_IMM
   | ARM_EOR_IMM
   | ARM_ORR_IMM
-  | ARM_BFM_IMM
-  | ARM_SBFM_IMM
+  | ARM_BFM_IMM 
+  | ARM_SBFM_IMM 
   | ARM_UBFM_IMM.
 (*Move (imm)*)
 Variant arm_move_imm :=
@@ -334,16 +308,16 @@ Variant arm_data_shifted :=
   | ARM_SUBS_SHIFTED_REG.
 
 Variant arm_log_shifted :=
-  | ARM_AND_LOG_REG
-  | ARM_ANDS_LOG_REG
-  | ARM_BIC_LOG_REG
-  | ARM_BICS_LOG_REG
-  | ARM_EON_LOG_REG
-  | ARM_EOR_LOG_REG
-  | ARM_ORR_LOG_REG
-  | ARM_MVN_LOG_REG
-  | ARM_ORN_LOG_REG
-  | ARM_TST_LOG_REG
+  | ARM_AND_LOG_REG 
+  | ARM_ANDS_LOG_REG 
+  | ARM_BIC_LOG_REG 
+  | ARM_BICS_LOG_REG 
+  | ARM_EON_LOG_REG 
+  | ARM_EOR_LOG_REG 
+  | ARM_ORR_LOG_REG 
+  | ARM_MVN_LOG_REG 
+  | ARM_ORN_LOG_REG 
+  | ARM_TST_LOG_REG 
   | ARM_MOV_LOG_REG.
 (*Add/Sub Extended*)
 Variant arm_extended :=
@@ -353,22 +327,22 @@ Variant arm_extended :=
   | ARM_SUBS_EXTENDED_REG.
 (*Add/Sub With Carry*)
 Variant arm_carry :=
-  | ARM_ADC
-  | ARM_ADCS
-  | ARM_SBC
+  | ARM_ADC 
+  | ARM_ADCS 
+  | ARM_SBC 
   | ARM_SBCS.
 (*Shift Register*)
 Variant arm_shift_reg :=
-  | ARM_ASRV_REG
-  | ARM_LSLV_REG
-  | ARM_LSRV_REG
+  | ARM_ASRV_REG 
+  | ARM_LSLV_REG 
+  | ARM_LSRV_REG 
   | ARM_RORV_REG.
 (*Bitops*)
 Variant arm_bitops :=
-  | ARM_CLS
-  | ARM_CLZ
-  | ARM_RBIT
-  | ARM_REV
+  | ARM_CLS  
+  | ARM_CLZ  
+  | ARM_RBIT 
+  | ARM_REV  
   | ARM_REV16
   | ARM_REV32
   | ARM_REV64.
@@ -380,7 +354,7 @@ Variant arm_load_gen :=
   | ARM_LDAPURH     | ARM_LDAPURSH
   | ARM_LDAPUR      | ARM_LDAPURSW
   | ARM_STLUR       | ARM_PRFM
-  | ARM_PRFM_IMM
+  | ARM_PRFM_IMM 
   (*load/store register (unscaled immediate)*)
   | ARM_STURB       | ARM_LDURB
   | ARM_LDURSB      | ARM_STURH
@@ -389,82 +363,82 @@ Variant arm_load_gen :=
   | ARM_LDURSW.
 (*Atomic*)
 Variant arm_atomic :=
-  | ARM_LDADDB      | ARM_LDCLRB
-  | ARM_LDEORB      | ARM_LDSETB
-  | ARM_LDSMAXB     | ARM_LDSMINB
-  | ARM_LDUMAXB     | ARM_LDUMINB
-  | ARM_SWPB        | ARM_LDADDH
-  | ARM_LDCLRH      | ARM_LDEORH
-  | ARM_LDSETH      | ARM_LDSMAXH
-  | ARM_LDSMINH     | ARM_LDUMAXH
+  | ARM_LDADDB      | ARM_LDCLRB 
+  | ARM_LDEORB      | ARM_LDSETB 
+  | ARM_LDSMAXB     | ARM_LDSMINB 
+  | ARM_LDUMAXB     | ARM_LDUMINB 
+  | ARM_SWPB        | ARM_LDADDH 
+  | ARM_LDCLRH      | ARM_LDEORH 
+  | ARM_LDSETH      | ARM_LDSMAXH 
+  | ARM_LDSMINH     | ARM_LDUMAXH 
   | ARM_LDUMINH     | ARM_SWPH
-  | ARM_LDADD       | ARM_LDCLR
-  | ARM_LDEOR       | ARM_LDSET
+  | ARM_LDADD       | ARM_LDCLR 
+  | ARM_LDEOR       | ARM_LDSET 
   | ARM_LDSMAX      | ARM_LDSMIN
   | ARM_LDUMAX      | ARM_LDUMIN
   | ARM_SWP         | ARM_LDAPRB
-  | ARM_LDAPRH      | ARM_LDAPR.
+  | ARM_LDAPRH      | ARM_LDAPR. 
 Variant arm_ldstr_reg :=
-  | ARM_STRB_REG
-  | ARM_LDRB_REG
-  | ARM_LDRSB_REG
-  | ARM_STRH_REG
-  | ARM_LDRH_REG
-  | ARM_LDRSH_REG
-  | ARM_STR_REG
-  | ARM_LDR_REG
-  | ARM_LDRSW_REG
+  | ARM_STRB_REG 
+  | ARM_LDRB_REG 
+  | ARM_LDRSB_REG 
+  | ARM_STRH_REG 
+  | ARM_LDRH_REG 
+  | ARM_LDRSH_REG 
+  | ARM_STR_REG 
+  | ARM_LDR_REG 
+  | ARM_LDRSW_REG 
   | ARM_PRFM_REG.
 Variant arm_unpriv :=
-  | ARM_STTRB
-  | ARM_LDTRB
-  | ARM_LDTRSB
-  | ARM_STTRH
-  | ARM_LDTRH
-  | ARM_LDTRSH
-  | ARM_STTR
-  | ARM_LDTR
-  | ARM_LDTRSW.
+  | ARM_STTRB 
+  | ARM_LDTRB 
+  | ARM_LDTRSB 
+  | ARM_STTRH 
+  | ARM_LDTRH 
+  | ARM_LDTRSH 
+  | ARM_STTR 
+  | ARM_LDTR 
+  | ARM_LDTRSW. 
 Variant arm_indexed :=
-  | ARM_STRB_IMM
-  | ARM_LDRB_IMM
-  | ARM_LDRSB_IMM
-  | ARM_LDR_IMM
-  | ARM_STRH_IMM
-  | ARM_LDRH_IMM
-  | ARM_LDRSH_IMM
-  | ARM_STR_IMM
-  | ARM_LDRSW_IMM.
+  | ARM_STRB_IMM 
+  | ARM_LDRB_IMM 
+  | ARM_LDRSB_IMM 
+  | ARM_LDR_IMM 
+  | ARM_STRH_IMM 
+  | ARM_LDRH_IMM 
+  | ARM_LDRSH_IMM 
+  | ARM_STR_IMM 
+  | ARM_LDRSW_IMM. 
 Variant arm_ld_reg_lit :=
-  | ARM_LDR_LIT
+  | ARM_LDR_LIT 
   | ARM_LDRSW_LIT
   | ARM_PRFM_LIT.
 Variant arm_ldstr_reg_pair :=
   | ARM_STP
   | ARM_LDP
   | ARM_LDPSW
-  | ARM_STGP.
+  | ARM_STGP. 
 Variant arm_exclusive :=
-  | ARM_STXRB       | ARM_STLXRB
-  | ARM_LDXRB       | ARM_LDXRH
-  | ARM_LDAXRB      | ARM_STLLRB
-  | ARM_STLLRH      | ARM_STLRH
-  | ARM_STLRB       | ARM_STXRH
+  | ARM_STXRB       | ARM_STLXRB 
+  | ARM_LDXRB       | ARM_LDXRH 
+  | ARM_LDAXRB      | ARM_STLLRB 
+  | ARM_STLLRH      | ARM_STLRH 
+  | ARM_STLRB       | ARM_STXRH 
   | ARM_STLXRH      | ARM_LDLARB
   | ARM_LDARB       | ARM_LDARH
-  | ARM_LDLARH      | ARM_STXR
-  | ARM_STLXR       | ARM_STXP
-  | ARM_STLXP       | ARM_LDXR
-  | ARM_LDAXR       | ARM_LDXP
+  | ARM_LDLARH      | ARM_STXR 
+  | ARM_STLXR       | ARM_STXP 
+  | ARM_STLXP       | ARM_LDXR 
+  | ARM_LDAXR       | ARM_LDXP 
   | ARM_LDAXP       | ARM_STLLR
   | ARM_STLR        | ARM_LDLAR
-  | ARM_LDAR        | ARM_CASP
+  | ARM_LDAR        | ARM_CASP 
   | ARM_CASB        | ARM_CASH
   | ARM_CAS         | ARM_LDAXRH.
 Variant inst :=
 (*DP imm*)
   | ARM_DATA_IMM (op: arm_add_sub_imm) (sf s sh imm12 Rn Rd : N)
-  (*v8.5: with tag, not implemented : ARM_ADDG, ARM_SUBG*)
+  (*v8.5: with tag, not implemented : ARM_ADDG, ARM_SUBG*)    
   | ARM_LOGICAL_IMM (op: arm_logical_imm) (Rn Rd immr imms sf n_:N)
   | ARM_MOVE_IMM (op: arm_move_imm) (Rd imm16 size shift:N)
   (*| TODO: ARM_MOV_IMM bitmask imm/wide imm/inverted wide imm*)
@@ -643,55 +617,156 @@ Variant inst :=
   | ARM_SETF8
   .
 
-(*  Returns an expression computing the highest set bit of 64-bit e.
-    Returns -1#64 if e is 0 (no bits are set). *)
-Definition HighestSetBit e := <{width(e)-1#64}>.
+(* Returns index in Xtemp[300], returns 0 for no-bits set, thus it is ambiguous.
+    Clobber Xtemp[301].
+
+    NB. We can embed HighestSetBit in a PIL expression rather than a statement
+    if we know the bitwidth beforehand. Just use a sequence of nested ites.
+    This already assumes a max iwdth of 64 bits. *)
+Definition HighestSetBit w e := <{
+  temp[301] := w#w - 1#w;
+  rep w#w do if (1#w<<Xtemp[301] & e) <> 0#w then nop else temp[301] := Xtemp[301] - 1#w end end;
+  temp[300] := Xtemp[301]
+}>.
+
+Print HighestSetBit.
 
 (* Return a w-bit expression of e ones *)
 Definition Ones w e := <{
   (1#w << e) - 1#w
 }>.
 
-(* Replicate M-bit x until the result is N bits.  N should be a multiple of M. *)
-Definition Replicate N M x :=
-  (N.iter (N.pred (N/M)) (fun acc => cbits acc M x) x) mod 2^N.
+Definition ROR w x shift := <{ite (shift#w = 0#w) x ((x >> shift#w) | (x << (w#w-shift#w)))}>.
 
-Definition ROR N shift x :=
-  let shift' := N.modulo shift N in 
-  N.lor (N.shiftr x shift') (N.shiftl x (N-shift')).
-
-(* shift < 2^w *)
-Definition RORExp w x shift := 
-  let m := <{shift#w % w#w}> in <{
-    ite (m = 0#w) x ((x >> m) | (x << (w#w-m)))
+(* Replicate w-bit expression x until it is w' bits *)
+Definition Replicate rettemp t w w' x := <{
+  if w'#w' % w#w' <> 0#w' then exn 0 else nop end;
+  temp[t] := 0#w;
+  temp[rettemp] := 0#w';
+  rep w'#w' / w#w' do temp[rettemp] := Xtemp[rettemp] | ((ucast w' x) << ((ucast w' Xtemp[t]) * w'#w')); temp[t] := Xtemp[t]+1#w end
 }>.
 
 (* J1-7389 *)
-(* Returns the wmask and tmask as a pair of M-bit Gallina Ns.
-   immN - 1 bit
-   imms, immr - 6 bit
-   M - output bitwidth*)
-Definition DecodeBitMasks (immN imms immr:N) (immediate:bool) (M:N) :=
-  let len := N.pred (N.size (cbits immN 6 (N.lnot imms 6))) in
-  match len, (N.shiftl 1 len) <=? M with
-  | 0, _ | _, false => (0,0)
-  | _, true =>
-      let levels := N.ones len (* 6-bit *) in
-      if immediate && ((N.land imms levels) =? levels) then (0,0) else
-      let S := N.land imms levels in
-      let R := N.land immr levels in
-      let diff := sbop2 Z.sub 6 S R in
-      let esize := N.shiftl 1 len in 
-      let d := xbits 0 len diff in
-      let welem := N.ones (S+1) in
-      let telem := N.ones (d+1) in
-      let welem' := ROR esize R welem in
-      let wmask := Replicate M esize welem' in
-      let tmask := Replicate M esize telem in
-      (wmask, tmask)
-  end.
-Definition wmask immN imms immr immediate M := fst (DecodeBitMasks immN imms immr immediate M).
-Definition tmask immN imms immr immediate M := snd (DecodeBitMasks immN imms immr immediate M).
+(* Writes the M-bit wmask and tmask into temp[980] and temp[990]. *)
+  Definition DecodeBitMasks (immN imms immr immediate M:N) :=
+    let imms := <{imms#6}> in
+    let immr := <{immr#6}> in
+    let immN := Word immN 1 in
+    let immediate := Word immediate 1 in
+    let immNNOTimms := <{immN ++ imms}> in
+    let levels := <{Xtemp[400]}> in
+    let S := <{Xtemp[401]}> in
+    let R := <{Xtemp[402]}> in
+    let lenw7 := <{Xtemp[300]}> in (* len <= 6 *)
+    let lenw6 := <{Xtemp[301]}> in (* len <= 6 *)
+    let esize := <{Xtemp[404]}> in
+    let d := <{Xtemp[405]}> in
+    <{
+      (* lenw7 *) 
+      temp[980] := 0#M;
+      temp[990] := 0#M;
+      {HighestSetBit 7 immNNOTimms};
+      (* The highest setbit position of w bits is w-1;
+          casting the len down to 6-bits does not lose information
+          and is useful below. *)
+      (* lenw6 *) temp[301] := lcast 6 lenw7;
+      if Xtemp[300] < 1#7 then exn 0 else nop end;
+      if 64#64 < (1#64 << ucast 64 Xtemp[300]) then exn 0 else nop end;
+
+      (* levels *) temp[400] := {Ones 6 lenw6};
+      if immediate & (imms & levels = levels) then exn 0 else nop end;
+      (* S *) temp[401] := imms & levels;
+      (* R *) temp[402] := immr & levels;
+      (* diff *) temp[403] := S-R;
+      (* esize *) temp[404] := 1#7 << lenw7;
+      (* d *) temp[405] := Xtemp[403] & levels;
+      if lenw6 = 1#6 then
+      (* wmask *) {Replicate 980 406 2 M <{{Ones 2 (Cast CAST_LOW 2 (BinOp OP_PLUS (Var (V_TEMP 401)) (Word 1 6)))}}>};
+      (* tmask *) {Replicate 990 406 2 M <{{Ones 2 <{lcast {2} ({d} + {1}#{6})}>}}>} else
+      if lenw6 = 2#6 then
+      (* wmask *) {Replicate 980 406 4 M <{{Ones 4 <{lcast {4} ({S} + {1}#{6})}>}}>};
+      (* tmask *) {Replicate 990 406 4 M <{{Ones 4 <{lcast {4} ({d} + {1}#{6})}>}}>} else
+      if lenw6 = 3#6 then
+      (* wmask *) {Replicate 980 406 8 M<{{Ones 8 <{ucast {8} ({S} + {1}#{6})}>}}>};
+      (* tmask *) {Replicate 990 406 8 M <{{Ones 8 <{ucast {8} ({d} + {1}#{6})}>}}>} else
+      if lenw6 = 4#6 then
+      (* wmask *) {Replicate 980 406 16 M <{{Ones 16 <{ucast {16} ({S} + {1}#{6})}>}}>};
+      (* tmask *) {Replicate 990 406 16 M <{{Ones 16 <{ucast {16} ({d} + {1}#{6})}>}}>} else
+      if lenw6 = 5#6 then
+      (* wmask *) {Replicate 980 406 32 M <{{Ones 32 <{ucast {32} ({S} + {1}#{6})}>}}>};
+      (* tmask *) {Replicate 990 406 32 M <{{Ones 32 <{ucast {32} ({d} + {1}#{6})}>}}>} else
+      if lenw6 = 6#6 then
+       {(if (M =? 64)%N then
+      <{
+        {Replicate 980 406 64 M <{{Ones 64 <{ucast {64} ({S} + {1}#{6})}>}}>};
+        {Replicate 990 406 64 M <{{Ones 64 <{ucast {64} ({d} + {1}#{6})}>}}>}
+      }>
+    else
+      <{ exn{0} }>
+    )}
+(**  (* wmask *) {Replicate 980 406 64 (if M=? 64 then ) <{{Ones 64 <{ucast {64} ({S} + {1}#{6})}>}}>};
+  (* tmask *) {Replicate 990 406 64 M <{{Ones 64 <{ucast {64} ({d} + {1}#{6})}>}}>}*)
+else
+  exn{0}
+end end end end end end
+  }>.
+
+    Definition DecodeBitMasks_32 (immN imms immr immediate:N) :=
+    let imms := <{imms#6}> in
+    let immr := <{immr#6}> in
+    let immN := Word immN 1 in
+    let immediate := Word immediate 1 in
+    let immNNOTimms := <{immN ++ imms}> in
+    let levels := <{Xtemp[400]}> in
+    let S := <{Xtemp[401]}> in
+    let R := <{Xtemp[402]}> in
+    let lenw7 := <{Xtemp[300]}> in (* len <= 6 *)
+    let lenw6 := <{Xtemp[301]}> in (* len <= 6 *)
+    let esize := <{Xtemp[404]}> in
+    let d := <{Xtemp[405]}> in
+    <{
+      (* lenw7 *) 
+      temp[980] := 0#32;
+      temp[990] := 0#32;
+      {HighestSetBit 7 immNNOTimms};
+      (* The highest setbit position of w bits is w-1;
+          casting the len down to 6-bits does not lose information
+          and is useful below. *)
+      (* lenw6 *) temp[301] := lcast 6 lenw7;
+      if Xtemp[300] < 1#7 then exn 0 else nop end;
+      if 32#64 < (1#64 << ucast 64 Xtemp[300]) then exn 0 else nop end;
+
+      (* levels *) temp[400] := {Ones 6 lenw6};
+      if immediate & (imms & levels = levels) then exn 0 else nop end;
+      (* S *) temp[401] := imms & levels;
+      (* R *) temp[402] := immr & levels;
+      (* diff *) temp[403] := S-R;
+      (* esize *) temp[404] := 1#7 << lenw7;
+      (* d *) temp[405] := Xtemp[403] & levels;
+      if lenw6 = 1#6 then
+      (* wmask *) {Replicate 980 406 2 32 <{{Ones 2 (Cast CAST_LOW 2 (BinOp OP_PLUS (Var (V_TEMP 401)) (Word 1 6)))}}>};
+      (* tmask *) {Replicate 990 406 2 32 <{{Ones 2 <{lcast {2} ({d} + {1}#{6})}>}}>} else
+      if lenw6 = 2#6 then
+      (* wmask *) {Replicate 980 406 4 32 <{{Ones 4 <{lcast {4} ({S} + {1}#{6})}>}}>};
+      (* tmask *) {Replicate 990 406 4 32 <{{Ones 4 <{lcast {4} ({d} + {1}#{6})}>}}>} else
+      if lenw6 = 3#6 then
+      (* wmask *) {Replicate 980 406 8 32<{{Ones 8 <{ucast {8} ({S} + {1}#{6})}>}}>};
+      (* tmask *) {Replicate 990 406 8 32 <{{Ones 8 <{ucast {8} ({d} + {1}#{6})}>}}>} else
+      if lenw6 = 4#6 then
+      (* wmask *) {Replicate 980 406 16 32 <{{Ones 16 <{ucast {16} ({S} + {1}#{6})}>}}>};
+      (* tmask *) {Replicate 990 406 16 32 <{{Ones 16 <{ucast {16} ({d} + {1}#{6})}>}}>} else
+      if lenw6 = 5#6 then
+      (* wmask *) {Replicate 980 406 32 32 <{{Ones 32 <{ucast {32} ({S} + {1}#{6})}>}}>};
+      (* tmask *) {Replicate 990 406 32 32 <{{Ones 32 <{ucast {32} ({d} + {1}#{6})}>}}>} else
+      
+  exn{0}
+end end end end end 
+  }>.
+
+  (* (* welem *) temp[410] := {Ones 64 <{ucast {64} ({S} + {1}#{6})}>};
+      (* telem *) temp[411] := {Ones 64 <{ucast {64} ({d} + {1}#{6})}>};
+      (* wmask *) {Replicate 980 406 64 64 <{Xtemp[410]}>};
+      (* tmask *) {Replicate 990 406 64 64 <{Xtemp[411]}>} ;*)
 
 Section Decoder.
   Variable n : N.
@@ -719,51 +794,74 @@ Section Decoder.
     | "1  0  0" => ARM_DATA_IMM ARM_ADD_IMM sf s sh imm12 Rn Rd (* ADD (immediate) - 64-bit variant on page C6-761 *)
     | "1  0  1" => ARM_DATA_IMM ARM_ADDS_IMM sf s sh imm12 Rn Rd (* ADDS (immediate) - 64-bit variant on page C6-769 *)
     | "1  1  0" => ARM_DATA_IMM ARM_SUB_IMM sf s sh imm12 Rn Rd (* SUB (immediate) - 64-bit variant on page C6-1311 *)
-    | "1  1  1" => ARM_DATA_IMM ARM_SUBS_IMM sf s sh imm12 Rn Rd (* SUBS (immediate) - 64-bit variant on page C6-1321 *)
+    | "1  1  1" => ARM_DATA_IMM ARM_SUBS_IMM sf s sh imm12 Rn Rd (* SUBS (immediate) - 64-bit variant on page C6-1321 *)  
     else UDF end.
 
-  (* n = 0 \/ n = 1 *)
+(**  (*immediate, with tags*)
+  Definition add_sub_imm_tags :=
+    let sf := n.[31] in
+    let op := n.[30] in
+    let s_ := n.[29] in
+    match[bits] sf, op, s_ with
+    | "0  -  -" => UDF (* Unallocated. - *)
+    | "1  -  1" => UDF (* Unallocated. - *)
+    | "1  0  0" => ARM_ADDG (* ADDG Armv8.5 *)
+    | "1  1  0" => ARM_SUBG (* SUBG Armv8.5 *)
+    else UDF end. *)
+
   Definition arm_ands_imm2il (Xn Xd immr imms sf n:N) :=
-    if (sf =? 0) && (n =? 1) then None else
+    let bit32variant := <{sf#1 = 0#1 & n#1 = 0#1}> in
     let datasize := (if sf =? 1 then 64 else 32) in
-    let imm := wmask n imms immr true datasize in
-    let operand1 := <{lcast datasize X[Xn]}> in
-    let result := <{ucast 64 (operand1 & imm#datasize)}> in
-    Some <{
-      var[Xd] := result;
-      R_NG := result[{datasize-1}];
-      R_ZR := result = 0#64;
+    let imm := <{Xtemp[980]}> in
+    let UNDEF := <{ (sf#1 = 0#1 & n#1 <> 0#1) }> in
+    <{
+      if UNDEF then exn 0 else nop end;
+      {DecodeBitMasks n imms immr 1 datasize};
+      (* imm: temp[980] *)
+      (* operand1 *) temp[1000] := lcast datasize X[Xn];
+      (* result *) {arm_varid Xd} := ucast 64 (Xtemp[1000] & imm);
+      R_NG := X[Xd][{datasize-1}];
+      R_ZR := X[Xd][0];
       R_CY := 0#1;
       R_OV := 0#1
     }>.
 
-  (* n = 0 \/ n = 1 *)
   Definition arm_and_imm2il (Xn Xd immr imms sf n:N) :=
-    if (sf =? 0) && (n =? 1) then None else
+    let bit32variant := <{sf#1 = 0#1 & n#1 = 0#1}> in
     let datasize := (if sf =? 1 then 64 else 32) in
-    let imm := wmask n imms immr true datasize in
-    let operand1 := <{lcast datasize X[Xn]}> in
-    Some <{
-       var[Xd] := ucast 64 (operand1 & imm#datasize)
+    let imm := <{Xtemp[980]}> in
+    let UNDEF := <{ (sf#1 = 0#1 & n#1 <> 0#1) }> in
+    <{
+      if UNDEF then exn 0 else nop end;
+      {DecodeBitMasks n imms immr 1 datasize};
+      (* imm: temp[980] *)
+      (* operand1 *) temp[1000] := lcast datasize X[Xn];
+       {arm_varid Xd} := ucast 64 (Xtemp[1000] & imm)
     }>.
 
   Definition arm_eor_imm2il (Xn Xd immr imms sf n:N) :=
-    if (sf =? 0) && (n =? 1) then None else
+    let bit32variant := <{sf#1 = 0#1 & n#1 = 0#1}> in
     let datasize := (if sf =? 1 then 64 else 32) in
-    let imm := wmask n imms immr true datasize in
-    let operand1 := <{lcast datasize X[Xn]}> in
+    let imm := <{Xtemp[980]}> in
     let UNDEF := <{ (sf#1 = 0#1 & n#1 <> 0#1) }> in
-    Some <{
-      var[Xd] := ucast 64 (operand1 ^ imm#datasize)
+    <{
+      if UNDEF then exn 0 else nop end;
+      {DecodeBitMasks n imms immr 1 datasize};
+      (* imm: temp[980] *) temp[1000] := lcast datasize X[Xn];
+      {arm_varid Xd} := ucast 64 (Xtemp[1000] ^ imm)
     }>.
 
-  Definition arm_orr_imm2il (Xn Xd immr imms sf n:N) :=
-    if (sf =? 0) && (n =? 1) then None else
+ Definition arm_orr_imm2il (Xn Xd immr imms sf n:N) :=
+    let bit32variant := <{sf#1 = 0#1 & n#1 = 0#1}> in
     let datasize := (if sf =? 1 then 64 else 32) in
-    let imm := wmask n imms immr true datasize in
-    let operand1 := <{lcast datasize X[Xn]}> in
-    Some <{
-      var[Xd] := ucast 64 (operand1 | imm#datasize)
+    let imm := <{Xtemp[980]}> in
+    let UNDEF := <{ (sf#1 = 0#1 & n#1 <> 0#1) }> in
+    <{
+      if UNDEF then exn 0 else nop end;
+      {DecodeBitMasks n imms immr 1 datasize};
+      (* imm: temp[980] *)
+      temp[1000] := lcast datasize X[Xn];
+      {arm_varid Xd} := ucast 64 (Xtemp[1000] | imm)
     }>.
 
   (*logical imm*)
@@ -843,47 +941,62 @@ Section Decoder.
       In both cases the destination bits below and above the bitfield are set to zero *)
 
   Definition arm_ubfm_imm2il (Xn Xd immr imms sf n:N) :=
-    if (sf =? 1) && negb (n =? 1) then None else
-    if (sf =? 0) && ((negb (n =? 0)) || (negb ((xbits immr 5 6)=?0)) || (negb ((xbits imms 5 6) =? 0))) then None else
+    let bit32variant := <{sf#1 = 0#1 & n#1 = 0#1}> in
     let datasize := (if sf =? 1 then 64 else 32) in
-    let R := Word immr datasize in
-    let wmask := wmask n imms immr false datasize in
-    let tmask := tmask n imms immr false datasize in
-    let src := <{lcast datasize X[Xn]}> in
-    let bot := <{{RORExp datasize src immr} & wmask#datasize}> in
-    Some <{
-      var[Xd] := ucast 64 (bot & tmask#datasize)
+    let wmask := <{Xtemp[980]}> in
+    let tmask := <{Xtemp[990]}> in
+    let UNDEF := <{ (sf#1 = 1#1 & n#1 <> 1#1) |
+                    ((sf#1 = 0#1) & (n#1 <> 0#1 | (immr#6 [5] <> 0#1) | (imms#6[5] <> 0#1))) }> in
+    <{
+      if UNDEF then exn 0 else nop end;
+      {DecodeBitMasks n imms immr 0 datasize};
+      (* wmask: temp[980]; tmask: temp[990] *)
+      (* src *) temp[1000] := X[Xn];
+      (* bot *) temp[1001] := {ROR datasize <{Xtemp[1000]}> immr} & wmask;
+      {arm_varid Xd} := Xtemp[1001] & tmask
     }>.
 
   Definition arm_bfm_imm2il (Xn Xd immr imms sf n:N) :=
-    if (sf =? 1) && negb (n =? 1) then None else
-    if (sf =? 0) && ((negb (n =? 0)) || (negb ((xbits immr 5 6)=?0)) || (negb ((xbits imms 5 6) =? 0))) then None else
+    let bit32variant := <{sf#1 = 0#1 & n#1 = 0#1}> in
     let datasize := (if sf =? 1 then 64 else 32) in
-    let wmask := wmask n imms immr false datasize in
-    let tmask := tmask n imms immr false datasize in
-    let dst := <{lcast datasize X[Xd]}> in
-    let src := <{lcast datasize X[Xn]}> in
-    let bot := <{(dst & {N.lnot wmask datasize}#datasize) 
-                  | ({RORExp datasize src immr} & wmask#datasize)}> in
-    Some <{
-      var[Xd] := ucast 64 ((dst & !tmask#datasize) | (bot & tmask#datasize))
+    let wmask := <{Xtemp[980]}> in
+    let tmask := <{Xtemp[990]}> in
+    let dst := <{Xtemp[1000]}> in
+    let bot := <{Xtemp[3000]}> in
+    let UNDEF := <{ (sf#1 = 1#1 & n#1 <> 1#1) |
+                    ((sf#1 = 0#1) & (n#1 <> 0#1 | (immr#6 [5] <> 0#1) | (imms#6[5] <> 0#1))) }> in
+    <{
+      if UNDEF then exn 0 else nop end;
+      {DecodeBitMasks n imms immr 0 datasize};
+      (* wmask: temp[980]; tmask: temp[990] *)
+      (* dst *) temp[1000] := lcast datasize X[Xd];
+      (* src *) temp[2000] := lcast datasize X[Xn];
+      (* bot *) temp[3000] := (dst & !wmask) | ({ROR datasize <{Xtemp[2000]}> immr} & wmask);
+      {arm_varid Xd} := ucast 64 ((dst * !tmask) | (bot & tmask))
+      (*{arm_varid Xd} := ucast 64 ((Xtemp[1000] * !tmask) | (Xtemp[3000] & tmask))*)
     }>.
 
   Definition pilxbits (w:N) (n lo hi:exp) :=
     <{ (n >> lo) % (1#w << (hi-lo)) }>.
 
   Definition arm_sbfm_imm2il (Xn Xd immr imms sf n:N) :=
-    if (sf =? 1) && negb (n =? 1) then None else
-    if (sf =? 0) && ((negb (n =? 0)) || (negb ((xbits immr 5 6)=?0)) || (negb ((xbits imms 5 6) =? 0))) then None else
+    let bit32variant := <{sf#1 = 0#1 & n#1 = 0#1}> in
     let datasize := (if sf =? 1 then 64 else 32) in
-    let wmask := wmask n imms immr false datasize in
-    let tmask := tmask n imms immr false datasize in
-    let src := <{lcast datasize X[Xn]}> in
-    let topbit := (if sf =? 0 then Word 0 1 else <{src[imms]}>) in
-    let bot := <{ {RORExp datasize src immr} & wmask#datasize }> in
-    let top := <{ite topbit ({N.ones datasize}#datasize) (0#datasize)}> in 
-    Some <{
-      var[Xd] := ucast 64 ((top & !tmask#datasize) | (bot & tmask#datasize))
+    let wmask := <{Xtemp[980]}> in
+    let tmask := <{Xtemp[990]}> in
+    let src := <{Xtemp[2000]}> in
+    let bot := <{Xtemp[3000]}> in
+    let top := <{Xtemp[4000]}> in
+    let UNDEF := <{ (sf#1 = 1#1 & n#1 <> 1#1) |
+                    ((sf#1 = 0#1) & (n#1 <> 0#1 | (immr#6 [5] <> 0#1) | (imms#6[5] <> 0#1))) }> in
+    <{
+      if UNDEF then exn 0 else nop end;
+      {DecodeBitMasks n imms immr 0 datasize};
+      (* wmask: temp[980]; tmask: temp[990] *)
+      (* src *) temp[2000] := lcast datasize X[Xn];
+      (* bot *) temp[3000] := {ROR datasize <{Xtemp[2000]}> immr} & wmask;
+      (* top *) {Replicate 4000 4001 1 64 (pilxbits datasize src (Word 0 datasize) (Word 1 datasize))};
+      {arm_varid Xd} := ucast 64 ((top & !tmask) | (bot & tmask))
     }>.
 
   Definition bitfield :=
@@ -1516,7 +1629,7 @@ Section Decoder.
 
   Definition arm_stxr2il_size (size Xn Xs Xt:N) :=
     let constraint1 := <{Xs#5 = Xt#5}> in
-    let constraint2 := <{(Xs#5 = Xn#5) & (Xn#5 <> 31#5)}> in <{
+    let constraint2 := <{Xs#5 = Xn#5 & Xn#5 <> 31#5}> in <{
       if ! constraint1 & ! constraint2 then {arm_stxr2il_constr size Xn Xs Xt (Word 0 1) (Word 0 1)} else
       if constraint1 then
         if unknown 1 then
@@ -1592,8 +1705,8 @@ Section Decoder.
     }>.
 
   Definition arm_stxp2il_size (size Xn Xs Xt Xt2:N) :=
-    let constraint1 := <{(Xs#5 = Xt#5) | (Xs#5 = Xt2#5)}> in
-    let constraint2 := <{(Xs#5 = Xn#5) & (Xn#5 <> 31#5)}> in <{
+    let constraint1 := <{Xs#5 = Xt#5 | Xs#5 = Xt2#5}> in
+    let constraint2 := <{Xs#5 = Xn#5 & Xn#5 <> 31#5}> in <{
       if ! constraint1 & ! constraint2 then {arm_stxp2il_constr size Xn Xs Xt Xt2 (Word 0 1) (Word 0 1)} else
       if constraint1 then
         if unknown 1 then
@@ -1954,7 +2067,7 @@ Section Decoder.
   Definition arm_ldp2il_constr Xn Xt Xt2 imm7 scale wback wb_unknown rt_unknown postindex :=
     let size := N.shiftl 8 scale in
     let dbytes := N.shiftl 1 scale in
-    let offset := <{scast 64 (imm7#64) << (scale # 64)}> in <{
+    let offset := <{scast 64 (imm7#7) << (scale # 64)}> in <{
       if (Xn # 5) = (31 # 5) then CheckSPAlignment else nop end; temp[1000] := X[Xn];
       if !{b2exp postindex} then temp[1000] := Xtemp[1000] + offset else nop end;
       temp[2000] := load[Xtemp[1000],LittleE,dbytes];
@@ -2021,7 +2134,7 @@ Section Decoder.
       else nop end}>.
 
   Definition arm_ldpsw2il_constr Xn Xt Xt2 imm7 wback wb_unknown rt_unknown postindex :=
-    let offset := <{scast 64 (imm7#64) << (2#64)}> in <{
+    let offset := <{scast 64 (imm7#7) << (2#64)}> in <{
       if (Xn # 5) = (31 # 5) then CheckSPAlignment else nop end; temp[1000] := X[Xn];
       if !{b2exp postindex} then temp[1000] := Xtemp[1000] + offset else nop end;
       temp[2000] := load[Xtemp[1000],LittleE,4];
@@ -2284,8 +2397,8 @@ Section Decoder.
       temp[2000] := X[Xt];
       if rtunknown then temp[2000] := ucast 64 unknown 8 else nop end;
       store[Xtemp[1000],Xtemp[2000],1];
-      temp[1001] := Xtemp[1000];
       if wback then
+        temp[1001] := Xtemp[1000];
         if postindex then temp[1001] := Xtemp[1001] + offset else nop end;
         var[Xn] := Xtemp[1001]
       else
@@ -2317,8 +2430,8 @@ Section Decoder.
       temp[2000] := X[Xt];
       if rtunknown then temp[2000] := ucast 64 unknown 16 else nop end;
       store[Xtemp[1000],Xtemp[2000],2];
-        temp[1001] := Xtemp[1000];
       if wback then
+        temp[1001] := Xtemp[1000];
         if postindex then temp[1001] := Xtemp[1001] + offset else nop end;
         var[Xn] := Xtemp[1001]
       else
@@ -2352,8 +2465,8 @@ Section Decoder.
       temp[2000] := X[Xt];
       if rtunknown then temp[2000] := ucast 64 unknown size else nop end;
       store[Xtemp[1000],Xtemp[2000],bytes];
-      temp[1001] := Xtemp[1000];
       if wback then
+        temp[1001] := Xtemp[1000];
         if postindex then temp[1001] := Xtemp[1001] + offset else nop end;
         var[Xn] := Xtemp[1001]
       else
@@ -2384,8 +2497,8 @@ Section Decoder.
       if (Xn # 5) = (31 # 5) then CheckSPAlignment else nop end; temp[1000] := X[Xn];
       if !postindex then temp[1000] := Xtemp[1000] + offset else nop end;
       var[Xt] := ucast 64 load[Xtemp[1000],1];
-      temp[1001] := Xtemp[1000];
       if wback & !wbsuppress then
+        temp[1001] := Xtemp[1000];
         if wbunknown then temp[1001] := unknown 64 else
         if postindex then temp[1001] := Xtemp[1001] + offset
         else nop end end;
@@ -2420,8 +2533,8 @@ Section Decoder.
       if (Xn # 5) = (31 # 5) then CheckSPAlignment else nop end; temp[1000] := X[Xn];
       if !postindex then temp[1000] := Xtemp[1000] + offset else nop end;
       var[Xt] := ucast 64 load[Xtemp[1000],2];
-      temp[1001] := Xtemp[1000];
       if wback & !wbsuppress then
+        temp[1001] := Xtemp[1000];
         if wbunknown then temp[1001] := unknown 64 else
         if postindex then temp[1001] := Xtemp[1001] + offset
         else nop end end;
@@ -2457,8 +2570,8 @@ Section Decoder.
       if (Xn # 5) = (31 # 5) then CheckSPAlignment else nop end; temp[1000] := X[Xn];
       if !postindex then temp[1000] := Xtemp[1000] + offset else nop end;
       var[Xt] := ucast 64 load[Xtemp[1000],bytes];
-      temp[1001] := Xtemp[1000];
       if wback & !wbsuppress then
+        temp[1001] := Xtemp[1000];
         if wbunknown then temp[1001] := unknown 64 else
         if postindex then temp[1001] := Xtemp[1001] + offset
         else nop end end;
@@ -2493,8 +2606,8 @@ Section Decoder.
       if (Xn # 5) = (31 # 5) then CheckSPAlignment else nop end; temp[1000] := X[Xn];
       if !postindex then temp[1000] := Xtemp[1000] + offset else nop end;
       var[Xt] := ucast 64 (scast size load[Xtemp[1000],1]);
-      temp[1001] := Xtemp[1000];
       if wback & !wbsuppress then
+        temp[1001] := Xtemp[1000];
         if wbunknown then temp[1001] := unknown 64 else
         if postindex then temp[1001] := Xtemp[1001] + offset
         else nop end end;
@@ -2529,8 +2642,8 @@ Section Decoder.
       if (Xn # 5) = (31 # 5) then CheckSPAlignment else nop end; temp[1000] := X[Xn];
       if !postindex then temp[1000] := Xtemp[1000] + offset else nop end;
       var[Xt] := ucast 64 (scast size load[Xtemp[1000],2]);
-      temp[1001] := Xtemp[1000];
       if wback & !wbsuppress then
+        temp[1001] := Xtemp[1000];
         if wbunknown then temp[1001] := unknown 64 else
         if postindex then temp[1001] := Xtemp[1001] + offset
         else nop end end;
@@ -2565,8 +2678,8 @@ Section Decoder.
       if (Xn # 5) = (31 # 5) then CheckSPAlignment else nop end; temp[1000] := X[Xn];
       if !postindex then temp[1000] := Xtemp[1000] + offset else nop end;
       var[Xt] := scast 64 load[Xtemp[1000],4];
-      temp[1001] := Xtemp[1000];
       if wback & !wbsuppress then
+        temp[1001] := Xtemp[1000];
         if wbunknown then temp[1001] := unknown 64 else
         if postindex then temp[1001] := Xtemp[1001] + offset
         else nop end end;
@@ -3194,8 +3307,8 @@ Section Decoder.
       if (Xn # 5) = (31 # 5) then CheckSPAlignment else nop end; temp[1000] := X[Xn];
       temp[1000] := Xtemp[1000] + offset;
       var[Xt] := load[Xtemp[1000],8];
-      temp[1001] := Xtemp[1000];
       if wback & !wbsuppress then
+        temp[1001] := Xtemp[1000];
         if wbunknown then temp[1001] := unknown 64 else nop end;
         var[Xn] := Xtemp[1001]
       else
@@ -3872,19 +3985,19 @@ Section Decoder.
     | ARM_ORN_LOG_REG |ARM_MVN_LOG_REG  => arm_shiftc true false (fun a b => BinOp OP_OR a (UnOp OP_NOT b))
     | ARM_EOR_LOG_REG => arm_shiftc true false (fun a b => BinOp OP_XOR a b) (*TODO: EORS?*)
     | ARM_EON_LOG_REG => arm_shiftc true false (fun a b => BinOp OP_XOR a (UnOp OP_NOT b))
-
+  
     end.
 
   Definition arm_withcarry_2il op (sf Rm Rn Rd:N) :=
     (*assign function here -> completed in the op_il function*)
     let datasize := if sf =? 1 then 64 else 32 in
     let arm_addwithcarry := arm_data_r_with_carry sf Rm Rn Rd in
-    match op with
+    match op with 
     | ARM_ADC => arm_addwithcarry true false (fun a b _ => AddWithCarry datasize a b (Var R_CY))
     | ARM_ADCS => arm_addwithcarry true true (fun a b _ => AddWithCarry datasize a b (Var R_CY))
     | ARM_SBC => arm_addwithcarry true false (fun a b _ => AddWithCarry datasize a (UnOp OP_NOT b) (Var R_CY))
     | ARM_SBCS => arm_addwithcarry true true (fun a b _ => AddWithCarry datasize a (UnOp OP_NOT b) (Var R_CY))
-    end.
+    end.   
 
 (**  Definition arm_data_r_il_shft op (cond sf s shift Rm Rd:N) imm6 (Rn:N) :=
     let arm_addwithcarry := arm_data_r_addwithcarry cond sf s shift Rm imm6 Rn in
@@ -3944,7 +4057,7 @@ Section Decoder.
     (*if condition holds, nzcv final is the new flags from AddWithCarry else its just the value we read in*)
     let result64 := if sf =? 1 then result else Cast CAST_UNSIGNED 64 result in
     arm_data_il false true Rn result64 nzcv_final.
-
+  
   Definition arm_data_imm2il op sf s sh imm12 Rn Rd:=
   let datasize := if sf =? 1 then 64 else 32 in
   match op with
@@ -3966,7 +4079,7 @@ Section Decoder.
   end.
 
   Definition arm_mov_imm2il op Rd imm16 size shift :=
-  match op with
+  match op with 
   | ARM_MOVZ_IMM  => arm_movz_imm2il Rd imm16 size shift
   | ARM_MOVN_IMM  => arm_movn_imm2il Rd imm16 size shift
   | ARM_MOVK_IMM  => arm_movk_imm2il Rd imm16 size shift
@@ -3985,6 +4098,199 @@ Section Decoder.
     | "x101" => dp_reg (* Data Processing -- Register on page C4-299 *)
     | "x111" => dp_fp_simd (* Data Processing -- Scalar Floating-Point and Advanced SIMD on page C4-309 *)
     else UDF end.
+
+  (*final arm2il-C6.2.5*)
+  Definition arm2il (a:addr) inst:=
+  let il := match inst with
+  (*DP imm*)
+  | ARM_DATA_IMM op sf s sh imm12 Rn Rd => arm_data_imm2il op sf s sh imm12 Rn Rd
+  (*logical imm*)
+  | ARM_LOGICAL_IMM op Rn Rd immr imms sf n_ => arm_log_imm2il op Rn Rd immr imms sf n_
+  (*move wide*)
+  | ARM_MOVE_IMM op Rd imm16 size shift => arm_mov_imm2il op Rd imm16 size shift
+  (*PC relative addressing*)
+(*| ARM_ADRP_IMM
+  | ARM_ADR_IMM *)
+  (*compare immediate*)
+  | ARM_CCMN_IMM sf Rn imm nzcv cond => arm_data_i_with_cond (ARM_CCMN_IMM sf Rn imm nzcv cond) sf Rn imm nzcv cond
+  | ARM_CCMP_IMM sf Rn imm nzcv cond => arm_data_i_with_cond (ARM_CCMP_IMM sf Rn imm nzcv cond) sf Rn imm nzcv cond
+  (*DP reg*)
+  (*arith extended*)
+  | ARM_EXTENDED op sf s opt Rm option_ imm3 Rn Rd => arm_extend_reg2il op 0 sf s Rm option_ imm3 Rn Rd
+  (*arith shifted*)
+  | ARM_DATA_SHIFTED op sf s shift Rm imm6 Rn Rd => arm_datashft_reg2il op 0 sf s shift Rm Rd imm6 Rn
+  (*logical shifted*)
+  | ARM_LOG_SHIFTED op sf shift Rm imm6 Rn Rd => arm_logshft_reg2il op 0 sf 0 shift Rm Rd imm6 Rn
+  (*carry operations*)
+  | ARM_CARRY op sf s Rm Rn Rd=> arm_withcarry_2il op sf Rm Rn Rd
+  (*shift register*)
+  | ARM_SHIFT _ sf Rm op2 Rn Rd => arm_data_r_shift_il sf Rm op2 Rn Rd true false
+  (*conditional comparison*)
+  | ARM_CCMN_REG sf Rm cond Rn nzcv=> arm_data_r_with_cond ARM_CCMN_REG_V cond sf Rm Rn nzcv
+  | ARM_CCMP_REG sf Rm cond Rn nzcv=> arm_data_r_with_cond ARM_CCMP_REG_V cond sf Rm Rn nzcv
+  (*rev*)
+  | ARM_BITOPS op sf Rn Rd => arm_data_rev_il op sf Rd
+  (*branch*)
+  | ARM_B_COND cond imm19 => arm_b_cond2il cond imm19
+  (*unconditional branch(register)*)
+  | ARM_BR Xn => arm_br2il Xn
+  | ARM_BLR Xn => arm_blr2il Xn
+  | ARM_RET Xn => arm_ret2il Xn
+  (*unconditional branch(imm)*)
+  | ARM_B imm26 => arm_b2il imm26
+  | ARM_BL imm26 => arm_bl2il imm26
+  (*compare and branch(imm)*)
+  | ARM_CBZ Rt imm19 size => arm_cbz2il Rt imm19 size
+  | ARM_CBNZ Rt imm19 size => arm_cbnz2il Rt imm19 size
+  (*test and branch(imm)*)
+  | ARM_TBZ Rt imm14 b5 b40 => arm_tbz2il Rt imm14 b5 b40
+  | ARM_TBNZ Rt imm14 b5 b40 => arm_tbnz2il Rt imm14 b5 b40
+(*Loads and Stores*)
+  (*exclusive/others*)
+  | ARM_EXCLUSIVE ARM_STXRB size Xn Xs Xt Xt2 => arm_stxrb2il Xn Xs Xt
+  | ARM_EXCLUSIVE ARM_STLXRB size Xn Xs Xt Xt2 => arm_stlxrb2il Xn Xs Xt
+  | ARM_EXCLUSIVE ARM_LDXRB size Xn Xs Xt Xt2 => arm_ldxrb2il Xn Xt 
+  | ARM_EXCLUSIVE ARM_LDXRH size Xn Xs Xt Xt2 => arm_ldxrh2il Xn Xt 
+  | ARM_EXCLUSIVE ARM_LDAXRH size Xn Xs Xt Xt2 => arm_ldaxrh2il Xn Xt
+  | ARM_EXCLUSIVE ARM_LDAXRB size Xn Xs Xt Xt2 => arm_ldaxrb2il Xn Xt
+  | ARM_EXCLUSIVE ARM_STLLRB size Xn Xs Xt Xt2 => arm_stllrb2il Xn Xt
+  | ARM_EXCLUSIVE ARM_STLLRH size Xn Xs Xt Xt2 => arm_stllrh2il Xn Xt
+  | ARM_EXCLUSIVE ARM_STLRH size Xn Xs Xt Xt2 => arm_stlrh2il Xn Xt
+  | ARM_EXCLUSIVE ARM_STLRB size Xn Xs Xt Xt2 => arm_stlrb2il Xn Xt
+  | ARM_EXCLUSIVE ARM_STXRH size Xn Xs Xt Xt2 => arm_stxrh2il Xn Xs Xt
+  | ARM_EXCLUSIVE ARM_STLXRH size Xn Xs Xt Xt2 => arm_stlxrh2il Xn Xs Xt
+  | ARM_EXCLUSIVE ARM_LDLARB size Xn Xs Xt Xt2 => arm_ldlarb2il Xn Xt
+  | ARM_EXCLUSIVE ARM_LDARB size Xn Xs Xt Xt2 => arm_ldarb2il Xn Xt
+  | ARM_EXCLUSIVE ARM_LDARH size Xn Xs Xt Xt2 => arm_ldarh2il Xn Xt
+  | ARM_EXCLUSIVE ARM_LDLARH size Xn Xs Xt Xt2 => arm_ldlarh2il Xn Xt
+  | ARM_EXCLUSIVE ARM_STXR size Xn Xs Xt Xt2 => arm_stxr2il size Xn Xs Xt 
+  | ARM_EXCLUSIVE ARM_STLXR size Xn Xs Xt Xt2 => arm_stxr2il_size size Xn Xs Xt
+  | ARM_EXCLUSIVE ARM_STXP size Xn Xs Xt Xt2 => arm_stxp2il size Xn Xs Xt Xt2
+  | ARM_EXCLUSIVE ARM_STLXP size Xn Xs Xt Xt2 => arm_stlxp2il size Xn Xs Xt Xt2 
+  | ARM_EXCLUSIVE ARM_LDXR size Xn Xs Xt Xt2 => arm_ldxr2il size Xn Xt
+  | ARM_EXCLUSIVE ARM_LDAXR size Xn Xs Xt Xt2 => arm_ldaxr2il size Xn Xt
+  | ARM_EXCLUSIVE ARM_LDXP size Xn Xs Xt Xt2 => arm_ldxp2il size Xn Xt Xt2
+  | ARM_EXCLUSIVE ARM_LDAXP size Xn Xs Xt Xt2 => havoc
+  | ARM_EXCLUSIVE ARM_STLLR size Xn Xs Xt Xt2 => arm_stllr2il size Xn Xt
+  | ARM_EXCLUSIVE ARM_STLR size Xn Xs Xt Xt2 => arm_stlr2il size Xn Xt
+  | ARM_EXCLUSIVE ARM_LDLAR size Xn Xs Xt Xt2 => arm_ldlar2il size Xn Xt
+  | ARM_EXCLUSIVE ARM_LDAR size Xn Xs Xt Xt2 => arm_ldar2il size Xn Xt
+  (*bunch of variants for these, refer to page C4-230*)
+  | ARM_EXCLUSIVE ARM_CASP size Xn Xs Xt Xt2 => arm_casp2il Xn Xs Xt size
+  | ARM_EXCLUSIVE ARM_CASB size Xn Xs Xt Xt2 => arm_casb2il Xn Xs Xt
+  | ARM_EXCLUSIVE ARM_CASH size Xn Xs Xt Xt2 => arm_cash2il Xn Xs Xt
+  | ARM_EXCLUSIVE ARM_CAS size Xn Xs Xt Xt2 => arm_cas2il Xn Xs Xt size
+  (*LDAPR/STLR unscaled immediate*)
+  | ARM_LOAD_GEN ARM_STLURB Xn Xt imm9 size => arm_stlurb2il Xn Xt imm9
+  | ARM_LOAD_GEN ARM_LDAPURB Xn Xt imm9 size => arm_ldapurb2il Xn Xt (Word imm9 64)
+  | ARM_LOAD_GEN ARM_LDAPURSB Xn Xt imm9 size => arm_ldapursb2il Xn Xt (Word imm9 64) size
+  | ARM_LOAD_GEN ARM_STLURH Xn Xt imm9 size => arm_stlurh2il Xn Xt (Word imm9 64) 
+  | ARM_LOAD_GEN ARM_LDAPURH Xn Xt imm9 size => arm_ldapurh2il Xn Xt (Word imm9 64)
+  | ARM_LOAD_GEN ARM_LDAPURSH Xn Xt imm9 size => arm_ldapursh2il Xn Xt (Word imm9 64) size
+  | ARM_LOAD_GEN ARM_LDAPUR Xn Xt imm9 size => arm_ldapur2il Xn Xt (Word imm9 64) size
+  | ARM_LOAD_GEN ARM_LDAPURSW Xn Xt imm9 size => arm_ldapursw2il Xn Xt (Word imm9 64) size
+  | ARM_LOAD_GEN ARM_STLUR Xn Xt imm9 size => arm_stlur2il Xn Xt (Word imm9 64) size
+  | ARM_LOAD_GEN ARM_PRFM Xn Xt imm9 size => arm_prfm_lit2il Xt imm9
+  | ARM_LOAD_GEN ARM_PRFM_IMM Xn Xt imm9 size => havoc
+  | ARM_ATOMIC ARM_LDAPRB size Xn Xs Xt => arm_ldaprb2il Xn Xt
+  | ARM_ATOMIC ARM_LDAPRH size Xn Xs Xt => arm_ldaprh2il Xn Xt
+  | ARM_ATOMIC ARM_LDAPR size Xn Xs Xt => arm_ldapr2il size Xn Xt
+  (*load/store memory tags*)
+  | ARM_STG Xn Xt imm9 writeback printindex => arm_stg2il Xn Xt imm9 writeback printindex
+  | ARM_STZG Xn Xt imm9 writeback printindex => arm_stzg2il Xn Xt imm9 writeback printindex
+  | ARM_STZGM Xn Xt => arm_stzgm2il Xt Xn         
+  | ARM_LDG Xn Xt imm9 => arm_ldg2il Xn Xt imm9
+  | ARM_ST2G Xn Xt imm9 writeback printindex => arm_st2g2il Xn Xt imm9 writeback printindex
+  | ARM_STGM Xn Xt => arm_stgm2il Xn Xt
+  | ARM_STZ2G Xn Xt imm9 writeback printindex => arm_stz2g2il Xn Xt imm9 writeback printindex
+  | ARM_LDGM Xn Xt => arm_ldgm2il Xn Xt
+  (*load register (literal)*)
+  | ARM_LD_REG_LIT ARM_LDR_LIT Xt imm19 size => arm_ldr_lit2il Xt imm19 size
+  | ARM_LD_REG_LIT ARM_LDRSW_LIT Xt imm19 size => arm_ldrsw_lit2il Xt imm19
+  | ARM_LD_REG_LIT ARM_PRFM_LIT Xt imm19 size => arm_prfm_lit2il Xt imm19
+  (*load/store no-allocate pair (offset)*)
+  | ARM_STNP Xn Xt Xt2 imm7 scale => arm_stnp2il Xn Xt Xt2 imm7 scale 
+  | ARM_LDNP Xn Xt Xt2 imm7 scale => arm_stnp2il Xn Xt Xt2 imm7 scale 
+  (*load/store register pair (post-indexed, pre-indexed, offset)*)
+  | ARM_LD_STR_REG_PAIR ARM_STP Xn Xt Xt2 imm7 scale wback postindex => arm_stp2il Xn Xt Xt2 imm7 scale wback postindex 
+  | ARM_LD_STR_REG_PAIR ARM_LDP Xn Xt Xt2 imm7 scale wback postindex => arm_ldp2il Xn Xt Xt2 imm7 scale wback postindex 
+  | ARM_LD_STR_REG_PAIR ARM_LDPSW Xn Xt Xt2 imm7 scale wback postindex => arm_ldpsw2il Xn Xt Xt2 imm7 wback postindex 
+  | ARM_LD_STR_REG_PAIR ARM_STGP Xn Xt Xt2 imm7 scale wback postindex => arm_stgp2il Xn Xt Xt2 imm7 wback postindex 
+  (*load/store register (unscaled immediate)*)
+  | ARM_LOAD_GEN ARM_STURB Xn Xt imm9 _ => arm_sturb2il Xn Xt imm9
+  | ARM_LOAD_GEN ARM_LDURB Xn Xt imm9 _ => arm_ldurb2il Xn Xt imm9
+  | ARM_LOAD_GEN ARM_LDURSB Xn Xt imm9 size => arm_ldursb2il Xn Xt imm9 size
+  | ARM_LOAD_GEN ARM_STURH Xn Xt imm9 _ => arm_sturh2il Xn Xt imm9
+  | ARM_LOAD_GEN ARM_LDURH Xn Xt imm9 _ => arm_ldurh2il Xn Xt imm9
+  | ARM_LOAD_GEN ARM_LDURSH Xn Xt imm9 size => arm_ldursh2il Xn Xt imm9 size
+  | ARM_LOAD_GEN ARM_STUR Xn Xt imm9 size => arm_stur2il Xn Xt imm9 size
+  | ARM_LOAD_GEN ARM_LDUR Xn Xt imm9 size => arm_ldur2il Xn Xt imm9 size
+  | ARM_LOAD_GEN ARM_LDURSW Xn Xt imm9 _ => arm_ldursw2il Xn Xt imm9
+  (*imm pre/post-indexed*)
+  | ARM_INDEXED ARM_STRB_IMM Xn Xt imm912 size signed wback postindex => arm_strb_imm2il Xn Xt imm912 signed wback postindex
+  | ARM_INDEXED ARM_LDRB_IMM Xn Xt imm912 size signed wback postindex => arm_ldrb_imm2il Xn Xt imm912 signed wback postindex 
+  | ARM_INDEXED ARM_LDRSB_IMM Xn Xt imm912 size signed wback postindex => arm_ldrsb_imm2il Xn Xt imm912 size signed wback postindex
+  | ARM_INDEXED ARM_LDR_IMM Xn Xt imm912 size signed wback postindex => arm_ldr_imm2il Xn Xt imm912 size signed wback postindex 
+  | ARM_INDEXED ARM_STRH_IMM Xn Xt imm912 size signed wback postindex => arm_strh_imm2il Xn Xt imm912 size signed wback postindex (*TODO: whats size?*)
+  | ARM_INDEXED ARM_LDRH_IMM Xn Xt imm912 size signed wback postindex => arm_ldrh_imm2il Xn Xt imm912 signed wback postindex
+  | ARM_INDEXED ARM_LDRSH_IMM Xn Xt imm912 size signed wback postindex => arm_ldrsh_imm2il Xn Xt imm912 size signed wback postindex
+  | ARM_INDEXED ARM_STR_IMM Xn Xt imm912 size signed wback postindex => arm_str_imm2il Xn Xt imm912 size signed wback postindex
+  | ARM_INDEXED ARM_LDRSW_IMM Xn Xt imm912 size signed wback postindex => arm_ldrsw_imm2il Xn Xt imm912 signed wback postindex
+  (*register unprivileged*)
+  | ARM_REG_UNPRIVILEGED ARM_STTRB Rn Rt imm9 size => arm_sttrb2il Rn Rt imm9
+  | ARM_REG_UNPRIVILEGED ARM_LDTRB Rn Rt imm9 size => arm_ldtrb2il Rn Rt imm9
+  | ARM_REG_UNPRIVILEGED ARM_LDTRSB Rn Rt imm9 size => arm_ldtrsb2il Rn Rt imm9 size
+  | ARM_REG_UNPRIVILEGED ARM_STTRH Rn Rt imm9 size => arm_sttrh2il Rn Rt imm9
+  | ARM_REG_UNPRIVILEGED ARM_LDTRH Rn Rt imm9 size => arm_ldtrh2il Rn Rt imm9
+  | ARM_REG_UNPRIVILEGED ARM_LDTRSH Rn Rt imm9 size => arm_ldtrsh2il Rn Rt imm9 size
+  | ARM_REG_UNPRIVILEGED ARM_STTR Rn Rt imm9 size => arm_sttr2il Rn Rt imm9 size
+  | ARM_REG_UNPRIVILEGED ARM_LDTR Rn Rt imm9 size => arm_ldtr2il Rn Rt imm9 size
+  | ARM_REG_UNPRIVILEGED ARM_LDTRSW Rn Rt imm9 size => arm_ldtrsw2il Rn Rt imm9 
+  (*atomic memory ops*)
+  | ARM_ATOMIC ARM_LDADDB size Xn Xs Xt => arm_ldaddb2il Xn Xs Xt
+  | ARM_ATOMIC ARM_LDCLRB size Xn Xs Xt => arm_ldclrb2il Xn Xs Xt
+  | ARM_ATOMIC ARM_LDEORB size Xn Xs Xt => arm_ldeorb2il Xn Xs Xt
+  | ARM_ATOMIC ARM_LDSETB size Xn Xs Xt => arm_ldsetb2il Xn Xs Xt
+  | ARM_ATOMIC ARM_LDSMAXB size Xn Xs Xt => arm_ldsmaxb2il Xn Xs Xt
+  | ARM_ATOMIC ARM_LDSMINB size Xn Xs Xt => arm_ldsminb2il Xn Xs Xt
+  | ARM_ATOMIC ARM_LDUMINB size Xn Xs Xt => arm_lduminb2il Xn Xs Xt
+  | ARM_ATOMIC ARM_SWPB size Xn Xs Xt => arm_swpb2il Xn Xs Xt
+  | ARM_ATOMIC ARM_LDADDH size Xn Xs Xt => arm_ldaddh2il Xn Xs Xt 
+  | ARM_ATOMIC ARM_LDCLRH size Xn Xs Xt => arm_ldclrh2il Xn Xs Xt
+  | ARM_ATOMIC ARM_LDEORH size Xn Xs Xt => arm_ldeorh2il Xn Xs Xt
+  | ARM_ATOMIC ARM_LDSETH size Xn Xs Xt => arm_ldseth2il Xn Xs Xt
+  | ARM_ATOMIC ARM_LDSMAXH size Xn Xs Xt => arm_ldsmaxh2il Xn Xs Xt
+  | ARM_ATOMIC ARM_LDSMINH size Xn Xs Xt => arm_ldsminh2il Xn Xs Xt
+  | ARM_ATOMIC ARM_LDUMAXH size Xn Xs Xt => arm_ldumaxh2il Xn Xs Xt
+  | ARM_ATOMIC ARM_LDUMINH size Xn Xs Xt => arm_lduminh2il Xn Xs Xt
+  | ARM_ATOMIC ARM_SWPH size Xn Xs Xt => arm_swph2il Xn Xs Xt
+  | ARM_ATOMIC ARM_LDADD size Xn Xs Xt => arm_ldadd2il size Xn Xs Xt
+  | ARM_ATOMIC ARM_LDCLR size Xn Xs Xt => arm_ldclr2il size Xn Xs Xt
+  | ARM_ATOMIC ARM_LDEOR size Xn Xs Xt => arm_ldeor2il size Xn Xs Xt
+  | ARM_ATOMIC ARM_LDSET size Xn Xs Xt => arm_ldset2il size Xn Xs Xt
+  | ARM_ATOMIC ARM_LDSMAX size Xn Xs Xt => arm_ldsmax2il size Xn Xs Xt
+  | ARM_ATOMIC ARM_LDSMIN size Xn Xs Xt => arm_ldsmin2il size Xn Xs Xt
+  | ARM_ATOMIC ARM_LDUMAX size Xn Xs Xt => arm_ldumax2il size Xn Xs Xt
+  | ARM_ATOMIC ARM_LDUMIN size Xn Xs Xt => arm_ldumin2il size Xn Xs Xt
+  | ARM_ATOMIC ARM_SWP size Xn Xs Xt => arm_swp2il size Xn Xs Xt
+  (*there's a lot more here, not sure how much to add. Pages C4-240-250*)
+  (*pac*)
+  | ARM_LDRAA Xn Xt s imm9 wback => arm_ldraa2il Xn Xt s imm9 wback
+  (*load/store register*)
+  | ARM_LD_STR_REG ARM_STRB_REG Xn Xm Xt extend _ _ => arm_strb_reg2il Xn Xm Xt extend
+  | ARM_LD_STR_REG ARM_LDRB_REG Xn Xm Xt extend _ _ => arm_ldrb_reg2il Xn Xm Xt extend
+  | ARM_LD_STR_REG ARM_LDRSB_REG Xn Xm Xt extend size _=> arm_ldrsb_reg2il Xn Xm Xt size extend
+  | ARM_LD_STR_REG ARM_STRH_REG Xn Xm Xt extend _ s => arm_strh_reg2il Xn Xm Xt extend s
+  | ARM_LD_STR_REG ARM_LDRH_REG Xn Xm Xt extend _ s => arm_ldrh_reg2il Xn Xm Xt extend s
+  | ARM_LD_STR_REG ARM_LDRSH_REG Xn Xm Xt extend size s => arm_ldrsh_reg2il Xn Xm Xt extend size s
+  | ARM_LD_STR_REG ARM_STR_REG Xn Xm Xt extend size s => arm_str_reg2il Xn Xm Xt extend size s
+  | ARM_LD_STR_REG ARM_LDR_REG Xn Xm Xt extend size s => arm_ldr_reg2il Xn Xm Xt extend size s
+  | ARM_LD_STR_REG ARM_LDRSW_REG Xn Xm Xt extend _ s => arm_ldrsw_reg2il Xn Xm Xt extend s
+ (* | ARM_LD_STR_REG ARM_PRFM_REG Xn Xm Xt extend _ s => havoc*)
+  | UDF => Exn 4
+  |_ => havoc end in
+  Seq (Move R_PC (Word (a mod 2^64) 64)) il.
+End Decoder.
 
 (********** well-typedness **********)
 Ltac destruct_match := repeat match goal with |- context [ match ?x with _ => _ end ] => destruct x end.
@@ -4105,22 +4411,7 @@ Proof.
   intros. unfold arm_varid. now destruct_match.
 Qed.
 
-Definition empty (v:var) : option N := None.
-
-Local Lemma pfsub_empty:
-  forall c, pfsub empty c.
-Proof.
-  intros; intros x y H; discriminate.
-Qed.
-
-Local Lemma hastyp_exp_empty:
-  forall c e n, hastyp_exp empty e n -> hastyp_exp c e n.
-Proof.
-  intros; eapply hastyp_exp_weaken;[eassumption | apply pfsub_empty].
-Qed.
-
 Require Import Lia ZifyN ZifyBool.
-Ltac Zify.zify_pre_hook ::= rewrite ?N.shiftl_mul_pow2, ?N.shiftr_div_pow2; unfold widthof_binop; (idtac + apply f_equal).
 
 Local Ltac etyp' :=
   repeat match goal with 
@@ -4181,7 +4472,7 @@ Local Ltac etyp :=
   | |- hastyp_exp _ (Cast _ _ _) _ => eapply TCast
 
   | |- match ?ct with | CAST_UNSIGNED => _ | _ => _ end => cbv; easy
-
+  
   (*| |- _ <= _ => easy lets see if it works*)
 
   | |- hastyp_exp _ (Var (arm_varid _)) 64 => apply hastyp_arm_varid
@@ -4194,7 +4485,6 @@ Local Ltac etyp :=
   | |- hastyp_exp _ (Store _ _ _ _ _) _ => apply TStore with (w := 64)
   | |- hastyp_exp _ (Extract ?hi ?lo ?e) ?n => replace n with (N.succ hi - lo);[eapply TExtract|]
   | X: hastyp_exp _ ?x ?a, Y: hastyp_exp _ ?y ?b |- hastyp_exp _ (Concat ?x ?y) _ => apply TConcat with (w1 := a) (w2 := b)
-  | H: hastyp_exp empty ?e _ |- hastyp_exp _ ?e _ => apply (hastyp_exp_empty _ _ _ H)
   | |- pfsub arm8typctx arm8typctx  => reflexivity
   | |- _ < _ => reflexivity
   | |- _ _ = Some _ => reflexivity
@@ -4210,6 +4500,7 @@ Local Ltac etypn size :=
   end.
 Local Ltac etyps size := repeat (etypn size + etyp).
 
+Print Move.
 Local Ltac stypc c :=
   cbn; repeat match goal with
          | |- hastyp_stmt _ _ (Seq _ _) _ => apply TSeq with (c1 := c) (c2 := c)
@@ -4228,30 +4519,10 @@ Local Ltac stypc c :=
          | |- hastyp_exp _ _ _  => etyp
   end.
 
-Local Ltac stypc_w c w' c1 c2 :=
-  cbn; repeat match goal with
-         | |- hastyp_stmt _ _ (Seq _ _) _ => apply TSeq with (c1 := c1) (c2 := c2)
-         | |- hastyp_stmt _ _ (If _ _   _) _ => apply TIf with (c2:=c2)
-         | |- hastyp_stmt _ _ (Exn _) _ => apply TExn
-         | |- hastyp_stmt _ _ (Rep _ _) _ => eapply TRep with (w:=w') (c:=c2)
-         | |- hastyp_stmt _ _ Nop _ => apply TNop
-         | |- hastyp_stmt _ _ (Jmp _) _ => apply TJmp with (w := 64)
-
-         | |- hastyp_stmt _ ?cx (Move (V_TEMP ?v) _) _ =>
-             apply TMove with (w := w') (c' := update c1 (V_TEMP v) (Some w'))
-
-         | |- hastyp_stmt _ _ (Move temp0 _) _ => apply TMove with (w := 64)
-         | |- hastyp_stmt _ _ (Move ?v _) _ => apply TMove with (w := sizeof v); [> right | | apply update_some]; try reflexivity
-         | |- pfsub armc armc  => reflexivity
-         | |- pfsub armc armct  => apply armct_sub
-         | |- hastyp_exp _ _ _  => etyp
-  end.
-
-
 Local Ltac e_stypc c :=
   (* Do not simplify the memory bitwidth and massage it into
      the TStore/TLoad format. *)
-  cbn -[N.mul N.pow N.shiftl N.shiftr]; rewrite ?(N.mul_comm 8 (2^64));
+  cbn -[N.mul N.pow]; rewrite ?(N.mul_comm 8 (2^64));
   repeat match goal with
   | |- hastyp_stmt _ _ (Seq _ _) _ => eapply TSeq
   | |- hastyp_stmt _ _ (If _ _ _) _ => eapply TIf
@@ -4317,12 +4588,12 @@ Lemma hastyp_arm_assign_flags:
     hastyp_exp armc flags 4 ->
     hastyp_stmt armc c (arm_assign_flags flags) armc.
 Proof.
-  intros. unfold arm_assign_flags.
-  destruct (Unpack_NZCV flags) as [[[? z] c0] v] eqn:Hunpack.
+  intros. unfold arm_assign_flags. 
+  destruct (Unpack_NZCV flags) as [[[n z] c0] v] eqn:Hunpack.
   pose proof (hastyp_Unpack_NZCV arm8typctx flags H0) as Hcomp.
   rewrite Hunpack in Hcomp. destruct Hcomp as [Hn [Hz [Hc0 Hc]]].
   styp; cbn; try eassumption. eapply hastyp_exp_weaken with (c1:= arm8typctx) (c2:=c); eassumption.
-Qed.
+Qed.  
 
 Lemma hastyp_AddWithCarry:
   forall c datasize x y carry_in,
@@ -4334,12 +4605,13 @@ Lemma hastyp_AddWithCarry:
     hastyp_exp c result datasize /\ hastyp_exp c nzcv 4.
 Proof.
   intros c datasize x y carry_in Hd Hx Hy Hcarry.
-  unfold AddWithCarry.
+  unfold AddWithCarry. 
   split.
   etyp; try eassumption. lia.
-  apply hastyp_Pack_NZCV.
-  all: etyp; try eassumption. all: try unfold widthof_binop. all: try lia.
+  apply hastyp_Pack_NZCV. 
+  all: etyp; try eassumption. all: try unfold widthof_binop. all: try lia. 
   all: try rewrite N.ones_equiv; apply N.lt_pred_l; apply N.pow_nonzero; try lia.
+
 Qed.
 
 Local Lemma hastyp_assign_R:
@@ -4348,9 +4620,9 @@ Local Lemma hastyp_assign_R:
     hastyp_exp armc e 64 ->
     hastyp_stmt armc c (arm_assign_R n e) armc.
 Proof.
-  intros. unfold arm_assign_R. styp.
+  intros. unfold arm_assign_R. styp. 
   rewrite sizeof_arm_varid. apply typeof_arm_varid.
-  rewrite sizeof_arm_varid.
+  rewrite sizeof_arm_varid. 
   apply hastyp_exp_weaken with (c1:= arm8typctx) (c2:= c);
   assumption.
   rewrite sizeof_arm_varid. apply typeof_arm_varid. assumption.
@@ -4397,15 +4669,15 @@ Ltac awc_branch32 e sh Rn:=
   destruct_match_rmr; destruct sh in e;
   try awc_sub_branch e;
   try first[reflexivity|assumption|left;reflexivity];
-  try apply TCast with (w:=32); try assumption; try lia;
-  try new_etyp; try reflexivity;try lia;
+  try apply TCast with (w:=32); try assumption; try lia; 
+  try new_etyp; try reflexivity;try lia; 
   try destruct (Rn=?31) eqn:Hrn;
   try new_etyp; try rewrite sizeof_arm_varid; try apply typeof_arm_varid; try reflexivity; try lia.
 
 Ltac awc sf Rn sh:=
   unfold_stmt; destruct (sf =? 1) eqn:?; destruct (Rn =? 31) eqn:?;
-  destruct_match_rmr;
-  match goal with
+  destruct_match_rmr; 
+  match goal with 
   | e: _ = (_,_) |- _ => awc_branch32 e sh Rn
   end.
 
@@ -4419,15 +4691,15 @@ Proof.
   - unfold_stmt. destruct (sf =? 1) eqn:?. destruct (Rn =? 31) eqn:?.
   + awc_branch e sh.
   + awc_branch e sh.
-  + awc_branch32 e sh Rn.
+  + awc_branch32 e sh Rn. 
   - unfold_stmt. destruct (sf =? 1) eqn:?. destruct (Rn =? 31) eqn:?.
   + awc_branch e sh.
   + awc_branch e sh.
-  + awc_branch32 e sh Rn.
+  + awc_branch32 e sh Rn. 
   - unfold_stmt. destruct (sf =? 1) eqn:?. destruct (Rn =? 31) eqn:?.
   + awc_branch e sh.
   + awc_branch e sh.
-  + awc_branch32 e sh Rn.
+  + awc_branch32 e sh Rn. 
   - unfold_stmt. destruct (sf =? 1) eqn:?. destruct (Rn =? 31) eqn:?.
   + awc_branch e sh.
   + awc_branch e sh.
@@ -4472,7 +4744,7 @@ Local Ltac solve_armc_sub :=
   match goal with
   | |- ?c ⊆ update ?c' ?x (Some ?y) =>
       first
-        [ apply update_some;  [ reflexivity||apply typeof_arm_varid | solve_armc_sub ]
+        [ apply update_some;  [ reflexivity | solve_armc_sub ]
         | apply update_fresh2; [ reflexivity | solve_armc_sub ]]
   | |- update ?c _ None ⊆ ?c2 => apply pfsub_remove
   | |- ?c ⊆ ?c2 => reflexivity || assumption
@@ -4494,11 +4766,44 @@ Local Ltac solve_armc_sub' :=
   end.
 
 
-Local Lemma Replicate_bound:
-  forall N0 M x, Replicate N0 M x < 2^N0.
+  Local Lemma hastyp_Replicate:
+  forall rettemp t w w' c x,
+    armc ⊆ c ->
+    w <> 0 -> w' <> 0 -> w <= w' -> t <> rettemp ->
+      (update c (V_TEMP rettemp) (Some w')) (temp[ t]) = None ->
+       hastyp_exp (update c (V_TEMP rettemp) (Some w')) x w ->
+    hastyp_stmt armc c (Replicate rettemp t w w' x)
+       (update c (V_TEMP rettemp) (Some w')) .
 Proof.
-  intros.  unfold Replicate. apply N.mod_lt. lia.
-Qed.
+   (*Todo- now easier that DecodeBitMasks is done.*)
+   intros. unfold Replicate. assert(w' < 2 ^ w') by apply lt_pow2_lin.
+   all: estyp. all: try lia. all: try reflexivity.
+   all: try rewrite update_updated; unfold sizeof_c.
+   rewrite update_updated. reflexivity.
+   rewrite update_updated. estyp. 
+   rewrite update_swap. 
+   eapply hastyp_exp_weaken. eassumption. 
+   eapply update_fresh2. eassumption.
+   eapply pfsub_update. reflexivity.
+    congruence.
+   rewrite update_updated. rewrite update_swap. 
+   new_etyp. rewrite update_updated. 
+   unfold sizeof_c. rewrite update_updated. reflexivity.
+   unfold sizeof_c. rewrite update_updated. assumption.
+   congruence.
+   rewrite update_updated. rewrite update_swap. estyp. lia. congruence.
+   rewrite update_updated. unfold widthof_binop.
+   rewrite update_cancel. rewrite update_swap, update_updated. reflexivity. congruence.
+   assert (w < 2^w') by lia. assert (0<w) by lia. 
+   rewrite <- N.pow_0_r with (n:=2). eapply N.pow_lt_mono_r. lia. assumption. 
+   rewrite update_updated. unfold widthof_binop.
+   rewrite update_cancel. rewrite update_swap. rewrite update_cancel. reflexivity.
+   congruence. rewrite update_swap. eapply update_fresh2. eassumption.
+   eapply pfsub_update. reflexivity.
+    congruence. 
+Qed. 
+
+
 
 Local Lemma hastyp_ConditionHolds:
   forall c n (PFSUB: pfsub arm8typctx c),  n<2^4 -> hastyp_exp c (ConditionHolds n) 1.
@@ -4511,7 +4816,7 @@ Local Lemma hastyp_XtoVar:
   forall n c (PFSUB: pfsub arm8typctx c), n < 2^5 -> hastyp_exp c (XtoVar n) 64.
 Proof.
   intros. unfold XtoVar.
-  repeat destruct_match; econstructor; apply PFSUB; reflexivity.
+  etyp; try easy; etypeasy.
 Qed.
 
 Local Lemma hastyp_AllocationTagFromAddress:
@@ -4554,7 +4859,7 @@ Local Lemma hastyp_MemSingleWrite:
   sz < 2^64 -> hastyp_stmt armc c (MemSingleWrite a sz v) c.
 Proof.
   intros; unfold MemSingleWrite. stypc c. apply hastyp_AlignCheck.
-  all: try assumption || reflexivity.
+  all: try assumption || reflexivity. 
   apply TMove with (w := sizeof V_MEM64).
     right. 3: apply update_some. 3: apply PFSUB.
     all:try reflexivity. etyp; etypeasy.
@@ -4572,7 +4877,7 @@ Local Lemma hastyp_BranchTo:
   forall c t (T:hastyp_exp c t 64) (PFSUB:pfsub armc c), hastyp_stmt armc c (BranchTo 64 t) c.
 Proof.
   intros; unfold BranchTo, UsingAArch32.
-  stypc c; etypeasy; try apply lt_pow2_lin || eassumption || reflexivity.
+  stypc c; etypeasy; try apply lt_pow2_lin || eassumption || reflexivity. 
 Qed.
 
 Local Lemma hastyp_arm_cbnz2il:
@@ -4595,6 +4900,7 @@ Proof.
   unfold sizeof; simpl. lia.
 Qed.
 
+Print arm_br2il.
 Local Lemma hastyp_arm_br2il:
   forall c (Xn:N) (B:Xn < 2^5) (PF:pfsub armc c), hastyp_stmt armc c (arm_br2il Xn) c.
 Proof.
@@ -4670,62 +4976,153 @@ Proof.
   all: reflexivity.
 Qed.
 
-Local Lemma DecodeBitMasks_bound:
-  forall immN imms immr immediate M
-    (B1:immN=0\/immN=1) (B2:imms<2^6) (B3:immr<2^6) (B4:M=32\/M=64),
-    match DecodeBitMasks immN imms immr immediate M with
-    | (w, t) => w<2^M /\ t<2^M
-    end.
+Local Lemma hastyp_HighestSetBit:
+  forall w e c,
+    pfsub armc c ->
+    w <> 0 -> w <= 64 ->
+    armc(temp[301]) = c(temp[301]) ->
+    hastyp_exp c e w ->
+    hastyp_stmt armc c (HighestSetBit w e)
+      (update (update c (V_TEMP 301) (Some w)) (V_TEMP 300) (Some w)).
 Proof.
-  intros; unfold DecodeBitMasks.
-  destruct_match_rmr.
-  destruct_match_in e.
-  1,2,4: inversion e; subst; lia.
-  match type of e with
-  | (?a, ?b) = (?n0, ?n1) =>
-      assert (H1: n0 = a) by (inversion e; subst; reflexivity);
-      assert (H2: n1 = b) by (inversion e; subst; reflexivity);
-      subst n0 n1; clear e
-  end.
-  split; apply Replicate_bound.
+  intros. assert(w < 2 ^ w) by apply lt_pow2_lin.
+  unfold_stmt.
+  eapply TSeq.
+  eapply TMove. left. reflexivity.
+  eapply TBinOp. eapply TWord. assumption.
+  eapply TWord. lia.
+  reflexivity. 
+  eapply TSeq.
+  eapply TRep. unfold widthof_binop. eapply TWord. assumption.
+  reflexivity.
+  estyp. 
+  all: try unfold widthof_binop. all: try rewrite update_cancel. all: try lia; try reflexivity.
+  2: rewrite update_cancel; reflexivity. 
+
+  eapply hastyp_exp_weaken. eassumption. apply update_fresh. rewrite <- H2. reflexivity.
+  eapply TMove. left. reflexivity. 
+  etyp. reflexivity.  
 Qed.
 
-Local Lemma wmask_bound:
-  forall immN imms immr immediate M
-    (B1:immN=0\/immN=1) (B2:imms<2^6) (B3:immr<2^6) (B4:M=32\/M=64),
-    wmask immN imms immr immediate M < 2^M.
-Proof.
-  intros; unfold wmask. pose proof (H:=DecodeBitMasks_bound immN imms immr immediate M B1 B2 B3 B4).
-  remember (DecodeBitMasks _ _ _ _ _) eqn:Heqp. unfold DecodeBitMasks in Heqp. destruct_match_in Heqp.
-  all:subst p; try simpl; try lia.
-  apply Replicate_bound.
+
+Local Lemma hastyp_pilxbits:
+  forall w n lo hi c,
+  1< 2^w ->
+  pfsub armc c->
+  hastyp_exp c n w ->
+  hastyp_exp c lo w ->
+  hastyp_exp c hi w ->
+  hastyp_exp c (pilxbits w n lo hi) 64.
+Proof. 
+  intros. unfold pilxbits. etyp; assumption.
 Qed.
 
-Local Lemma hastyp_wmask:
-  forall immN imms immr immediate M
-    (B1:immN=0\/immN=1) (B2:imms<2^6) (B3:immr<2^6) (B4:M=32\/M=64),
-    hastyp_exp armc (Word (wmask immN imms immr immediate M) M) M.
-Proof.
-  intros; econstructor. apply wmask_bound; lia.
-Qed.
 
-Local Lemma tmask_bound:
-  forall immN imms immr immediate M
-    (B1:immN=0\/immN=1) (B2:imms<2^6) (B3:immr<2^6) (B4:M=32\/M=64),
-    tmask immN imms immr immediate M < 2^M.
+Local Lemma hastyp_DecodeBitMasks:
+  forall immN imms immr immediate M,
+    (immN < 2) -> (imms < 2^6) -> (immr < 2^6) ->
+    (immediate = 0 \/ immediate = 1) ->
+    (M=32 \/ M =64)->
+    hastyp_stmt armc armc (DecodeBitMasks immN imms immr immediate M) 
+    (update (update (update (update (update (update (update (update (update (update armc
+    (V_TEMP 301) (None))
+    (V_TEMP 300) (None))
+    (V_TEMP 400) (None))
+    (V_TEMP 401) (None))
+    (V_TEMP 402) (None))
+    (V_TEMP 403) (None))
+    (V_TEMP 404) (None))
+    (V_TEMP 405) (None))
+    (V_TEMP 990) (Some M))
+    (V_TEMP 980) (Some M)).
 Proof.
-  intros; unfold tmask. pose proof (H:=DecodeBitMasks_bound immN imms immr immediate M B1 B2 B3 B4).
-  remember (DecodeBitMasks _ _ _ _ _) eqn:Heqp. unfold DecodeBitMasks in Heqp. destruct_match_in Heqp.
-  all:subst p; try simpl; try lia.
-  apply Replicate_bound.
-Qed.
-
-Local Lemma hastyp_tmask:
-  forall immN imms immr immediate M
-    (B1:immN=0\/immN=1) (B2:imms<2^6) (B3:immr<2^6) (B4:M=32\/M=64),
-    hastyp_exp armc (Word (tmask immN imms immr immediate M) M) M.
-Proof.
-  intros; econstructor. apply tmask_bound; lia.
+  intros. unfold_stmt. 
+  estyp. lia. reflexivity. lia. reflexivity.
+  eapply hastyp_HighestSetBit. eapply update_fresh2. reflexivity.
+  eapply update_fresh2. reflexivity. reflexivity . 1-2: lia.
+  rewrite update_frame by congruence.
+  rewrite update_frame by congruence. reflexivity.
+  replace 7 with (1 + 6) by lia. eapply TConcat. etyp. assumption. etyp. assumption. reflexivity. 
+  all: try eapply hastyp_Ones.
+  all: try rewrite update_frame by congruence;
+  try rewrite update_updated; try reflexivity.
+  all: try unfold sizeof_c ;try rewrite update_updated; try lia.
+  rewrite update_swap. rewrite update_updated. lia.
+  congruence. 
+  rewrite update_swap. rewrite update_cancel.
+  rewrite update_swap. estyp. apply update_updated.
+  1-2: try congruence. 
+  all: try estyp; repeat (rewrite update_frame; [| congruence]); try apply update_updated.
+  - eapply hastyp_Replicate. solve_armc_sub. 1-4: lia. etyp. 
+  repeat rewrite update_frame by congruence. reflexivity.
+  eapply hastyp_Ones. lia. etyp. unfold widthof_binop. lia. 
+  - eapply hastyp_stmt_weaken'. eapply hastyp_Replicate.  solve_armc_sub. 1-4: lia. 
+    repeat rewrite update_frame by congruence. reflexivity.
+  eapply hastyp_Ones. lia. etyp. unfold widthof_binop. lia.  solve_armc_sub. 
+  - eapply hastyp_Replicate. solve_armc_sub. 1-4: lia. 
+    repeat rewrite update_frame by congruence. reflexivity.
+  eapply hastyp_Ones. lia. etyp. unfold widthof_binop. lia. 
+  - eapply hastyp_stmt_weaken' . eapply hastyp_Replicate. solve_armc_sub. 1-4: lia.
+    repeat rewrite update_frame by congruence. reflexivity.
+  eapply hastyp_Ones. lia. etyp. unfold widthof_binop. lia. solve_armc_sub.
+  - eapply hastyp_Replicate. solve_armc_sub. 1-4: lia.
+    repeat rewrite update_frame by congruence. reflexivity.
+  eapply hastyp_Ones. lia. etyp. unfold widthof_binop. lia. 
+  - eapply hastyp_stmt_weaken' . eapply hastyp_Replicate. solve_armc_sub. 1-4: lia.
+    repeat rewrite update_frame by congruence. reflexivity.
+  eapply hastyp_Ones. lia. etyp. unfold widthof_binop. lia. solve_armc_sub.
+  - eapply hastyp_Replicate. solve_armc_sub. 1-4: lia.
+    repeat rewrite update_frame by congruence. reflexivity.
+  eapply hastyp_Ones. lia. etyp. unfold widthof_binop. lia. 
+  - eapply hastyp_stmt_weaken' . eapply hastyp_Replicate. solve_armc_sub. 1-4: lia. 
+    repeat rewrite update_frame by congruence. reflexivity.
+  eapply hastyp_Ones. lia. etyp. unfold widthof_binop. lia. solve_armc_sub.
+  - eapply hastyp_Replicate. solve_armc_sub. 1-4: lia.
+    repeat rewrite update_frame by congruence. reflexivity.
+  eapply hastyp_Ones. lia. etyp. unfold widthof_binop. lia.  
+  - eapply hastyp_stmt_weaken' . eapply hastyp_Replicate. solve_armc_sub. 1-4: lia. 
+    repeat rewrite update_frame by congruence. reflexivity.
+  eapply hastyp_Ones. lia. etyp. unfold widthof_binop. lia. solve_armc_sub.
+  - destruct H3 as [|].
+  ++ subst. psimpl. estyp. solve_armc_sub.
+  ++ subst. 
+  estyp.
+   -- eapply hastyp_Replicate. solve_armc_sub. 1-4: try lia. 
+    repeat rewrite update_frame by congruence. reflexivity.
+  eapply hastyp_Ones. lia. etyp. unfold widthof_binop. lia. 
+   -- eapply hastyp_stmt_weaken'. 
+   eapply hastyp_Replicate. solve_armc_sub. 1-4: lia. 
+    repeat rewrite update_frame by congruence. reflexivity.
+  eapply hastyp_Ones. lia. etyp. unfold widthof_binop. lia. reflexivity.
+  -- solve_armc_sub.
+  - rewrite update_updated.
+    repeat rewrite update_swap with (x1:=temp[403]) (x2:=temp[404]) by congruence.
+    rewrite update_updated.
+    repeat rewrite update_swap with (x1:=temp[301]) (x2:=temp[300]) by congruence.
+    rewrite update_cancel.
+    rewrite update_swap with (x1:=temp[990]) (x2:=temp[300]) by congruence.
+    rewrite update_swap with (x1:=temp[990]) (x2:=temp[301]) by congruence.
+    rewrite update_swap with (x1:=temp[990]) (x2:=temp[400]) by congruence.
+    rewrite update_swap with (x1:=temp[990]) (x2:=temp[401]) by congruence.
+    rewrite update_swap with (x1:=temp[990]) (x2:=temp[402]) by congruence.
+    rewrite update_swap with (x1:=temp[990]) (x2:=temp[404]) by congruence.
+    rewrite update_swap with (x1:=temp[990]) (x2:=temp[403]) by congruence.
+    rewrite update_swap with (x1:=temp[980]) (x2:=temp[300]) by congruence.
+    rewrite update_swap with (x1:=temp[980]) (x2:=temp[301]) by congruence.
+    rewrite update_swap with (x1:=temp[980]) (x2:=temp[400]) by congruence.
+    rewrite update_swap with (x1:=temp[980]) (x2:=temp[401]) by congruence.
+    rewrite update_swap with (x1:=temp[980]) (x2:=temp[402]) by congruence.
+    rewrite update_swap with (x1:=temp[980]) (x2:=temp[404]) by congruence.
+    rewrite update_swap with (x1:=temp[980]) (x2:=temp[403]) by congruence.
+    rewrite update_swap with (x1:=temp[980]) (x2:=temp[990]) by congruence.
+    rewrite update_swap with (x1:=temp[980]) (x2:=temp[405]) by congruence.
+    rewrite update_swap with (x1:=temp[990]) (x2:=temp[405]) by congruence.
+    repeat apply pfsub_update.
+    intros x y PF.
+    repeat match goal with
+           |- update ?c ?v _ _= _ => destruct (iseq x v);[subst; (repeat rewrite update_frame in PF by intro;discriminate); rewrite update_updated in PF; discriminate| rewrite update_frame in * by assumption ]
+           end.
+    assumption.
 Qed.
 
 Local Lemma update_sub :
@@ -4758,11 +5155,6 @@ Proof.
   reflexivity.
 Qed.
 
-Local Lemma armvarid_neq_mem:
-  forall n, arm_varid n <> V_MEM64.
-Proof.
-  intros n0 EQ. pose proof (H:=typeof_arm_varid n0). now rewrite EQ in H.
-Qed.
 
 
 Local Ltac c_var :=
@@ -4779,7 +5171,6 @@ Proof.
     subst; rewrite update_updated in *; discriminate.
     assumption.
 Qed.
-
 
 (* Simplifies goals reading vars from a context that is a superset of armc. Example simplified expression:
 
@@ -4818,21 +5209,13 @@ Local Ltac red_ccases :=
   | _ => idtac
   end.
 
-(* [cget] solves or simplifies [c x = Some _] goals where c has updates and
-   maybe we need to appeal to a pfsub hypothesis. *)
-Local Ltac cget :=
-  rewrite ?update_frame by (discriminate||(idtac+symmetry);(apply armvarid_neq_temp + apply armvarid_neq_mem) ||intros H;inversion H;lia);
-  ((rewrite update_updated; try reflexivity)
-  || lazymatch goal with 
-     | H: pfsub armc ?c |- ?c _ = Some _ => apply H; simpl; try (reflexivity || apply typeof_arm_varid)
-     | H: pfsub ?c' ?c |- ?c _ = Some _ => apply H; cget
-     end).
-
 (* c_varx solves more complicated context equations like the one below:
 
 PF : arm8typctx ⊆ c
 H : (c[temp[ 1000] := None][temp[ 9000] := None]) x = Some y
+
 ========================= (1 / 1)
+
 (c[temp[ 9000] := Some 64][temp[ 1000] := Some 64][temp[ 1000] := Some 64]
  [V_MEM64 := Some (8 * 2 ^ 64)]) x = Some y *)
 Ltac c_varx :=
@@ -4844,7 +5227,6 @@ Ltac c_varx :=
   | H: ?x = Some _, H2: ?x = None |- _ => now rewrite H in H2
   (* Used when proving that armc is a satisfactory output context. *)
   | PF: pfsub armc ?c |- ?c _ = _ => apply PF; assumption
-  | PF: pfsub armc ?c |- Some _ = ?c _ => symmetry; apply PF; (reflexivity || assumption || apply typeof_arm_varid)
   | PF: pfsub armc ?c |- context[?c ?v] => rewrite (PF v _ (eq_refl _)); rewrite ?(N.mul_comm 8); reflexivity
   (* Reducers *)
   | PF:arm8typctx ⊆ _, EQ:?c' ?x = _ |- update ?c ?v  (Some ?val) ?x = Some ?y =>
@@ -4854,15 +5236,14 @@ Ltac c_varx :=
                 second case solves when the output context is weakend to arm8typctx.
                 The latter case is useful for simplifying and indicating the theorems for
                 terminal lifter code as opposed to internal auxiliary functions. *)
-            first [ assumption
-                  | specialize (PF v val eq_refl) || specialize (PF v val (typeof_arm_varid _));
+            first [ specialize (PF v val eq_refl) || specialize (PF v val (typeof_arm_varid _));
                     rewrite PF, <- EQ in *; reflexivity
                   | discriminate ||
                     match goal with | EQ: armc _ = Some ?y |- _ = Some ?y =>
                       rewrite <-EQ, ?typeof_arm_varid; reflexivity
                     end
                   ]
-         | rewrite ?update_frame in * by assumption ]
+          | rewrite update_frame by assumption ]
   | PF: pfsub armc _, EQ: ?c' ?x = _|- update ?c ?v (Some ?val) ?x = Some ?y => destruct (iseq x v);
       [subst;rewrite update_updated; (specialize (PF v val (eq_refl _)) || specialize (PF v val (typeof_arm_varid _))); rewrite PF, <-EQ in *; reflexivity
       |rewrite update_frame by assumption]
@@ -4870,12 +5251,6 @@ Ltac c_varx :=
       [subst;rewrite update_updated,?update_frame in * by (discriminate||apply armvarid_neq_temp||intros H;inversion H;lia);
          rewrite <-EQ
          |rewrite update_frame by assumption]
-  (* Adding this case breaks proofs. *)
-  (*| |- context[update ?c ?v (Some _) ?x] => *)
-  (*    rewrite (update_updated c x) ||*)
-  (*    let EQ:=fresh "EQ" in*)
-  (*    let NEQ:=fresh "NEQ" in*)
-  (*    destruct (x==v) as [EQ|NEQ];[rewrite EQ in *; clear EQ|rewrite ?(update_frame _ _ _ _ NEQ)]*)
   end.
 
 (* Prove pfsub goals. *)
@@ -4887,36 +5262,26 @@ Ltac subsolve :=
 
 (* Try to solve a hastyp_exp goal, dealing with fairly complex context subset subgoals. *)
 Local Ltac esolve :=
-  simpl_c; etyp; 
-  (apply hastyp_XtoVar
-    || apply hastyp_b2exp
-    || apply hastyp_AlignCheck
-    || idtac
-  ); try etypeasy; try solve_armc_sub; try c_var; try c_varx.
+  simpl_c; etyp; try apply hastyp_XtoVar; try etypeasy; try solve_armc_sub; try c_var; try c_varx.
 
 (* Try to solve a hastyp_stmt goal using aux-function lemmas. *)
-Local Ltac ssolve H :=
-    apply H
+Local Ltac ssolve :=
+  estyp
     || apply hastyp_havoc
     || apply hastyp_CheckSPAlignment
     || apply hastyp_BranchTo
     || apply hastyp_ExtendReg
-    (*|| apply Replicate_bound*)
-    || apply hastyp_wmask || apply hastyp_tmask
-    || estyp.
+    || apply hastyp_Replicate
+    || apply hastyp_HighestSetBit
+    || apply hastyp_DecodeBitMasks.
 
 Ltac destruct_oreq :=
   try match goal with
-  | H: ?x = _ \/ _ |- context[?x] => destruct H; subst
+  | H: ?x = _ \/ ?x = _ |- context[?x] => destruct H; subst
   end.
 
 Ltac casesolve := 
-  assumption 
-  (* Apply specific reflexivity lemmas.  Using [reflexivity] binds the evar in, e.g., [?w <= 64]
-     leading to unprovable goals. *)
-  || apply pfsub_refl || apply eq_refl
-  (* Subfunctions for DecodeBitMasks users (e.g. UBFM). *)
-  || (apply wmask_bound;lia) || (apply tmask_bound; lia)
+  assumption || apply pfsub_refl || apply eq_refl
   (* Some functions take the minimum of two values. *)
   || (apply N.min_le_iff; first [left;lia | right;lia])
   (* For N.shiftl 1 size <= 64 goals *)
@@ -4926,62 +5291,18 @@ Ltac casesolve :=
   (* pfsub *)
   || subsolve
   (* hastyp_exp *)
-  || esolve
-  (* context x = Some _ *)
-  || cget.
+  || esolve.
 
 (* Step through a hastyp_stmt proof, solving trivially solvable cases. *)
-Ltac econs_ H :=
+Ltac econs :=
   (* econstructor by default, but prefer special cases for TLoad and TStore
      to unify the memory bitwidth early and allow the solvers to solve the other
      goals. *)
   ( (eapply TLoad;[|etyp;casesolve|])
     || (eapply TStore;[|etyp;casesolve| | ])
-    || econstructor
-    || (rewrite N.mul_comm; econstructor));
+    || econstructor);
   simpl_c; repeat destruct_match;
-  try solve [(try ssolve H); (casesolve || (try destruct_oreq; repeat (try etyp; casesolve)))].
-
-(* `econs with H` gives econs a hint of how to solve subgoals after its
-   econstructor step. *)
-Tactic Notation "econs" "with" reference(h) := econs_ h.
-Tactic Notation "econs" := econs_ I.
-
-(* For solving fetching a register out of a big context.  E.g.,
-  (c[temp[ 1000] := Some 64][temp[ 2000] := Some (N.shiftl 1 scale * 8)]
-  [temp[ 3000] := Some (N.shiftl 1 scale * 8)][temp[ 2000] := Some (N.shiftl 8 scale)]
-  [temp[ 3000] := Some (N.shiftl 8 scale)][<{ var[ {Xt}] }> := Some 64]
-  [<{ var[ {Xt2}] }> := Some 64]) <{ var[ {Xn}] }> =
-    Some 64 *)
-Ltac c_var_reg :=
-repeat match goal with
-|- update ?c ?v ?val ?x = Some _ =>
-    (rewrite update_updated; reflexivity)
-    || (rewrite update_frame by (discriminate||((idtac+symmetry); apply armvarid_neq_temp)))
-    || (let EQ:=fresh "EQ" in destruct (x==v) as [EQ | ?];[rewrite <-EQ in *; rewrite update_updated; reflexivity | rewrite update_frame by assumption ])
-| PF: pfsub armc ?c |- ?c _ = Some _ => apply PF; try (reflexivity || apply typeof_arm_varid)
-end.
-
-Local Ltac simple_c_var :=
-  (idtac+symmetry);
-    (repeat match goal with
-    | |- update ?c (arm_varid ?v) _ (arm_varid ?x) = _ =>
-        let EQ := fresh "EQ" in 
-        destruct (arm_varid x == arm_varid v) as [EQ | ?];[
-            rewrite <-EQ,update_updated in *; clear EQ; try reflexivity
-            | rewrite update_frame by assumption
-            ]
-    | |- _ => rewrite !update_frame by
-          ((intros;discriminate) || (idtac+symmetry);(apply armvarid_neq_temp || apply armvarid_neq_mem))
-    end);
-    match goal with
-    | PF: pfsub armc ?c |- ?c _ = _ => apply PF, typeof_arm_varid
-    | |- armc _ = _ => reflexivity
-    end.
-    (*rewrite !update_frame by (apply armvarid_neq_temp || apply armvarid_neq_mem); *)
-    (*match goal with*)
-    (*| PF: pfsub armc ?c |- ?c _ = _ => apply PF, typeof_arm_varid*)
-    (*end.*)
+  try solve [(try ssolve); (casesolve || (try destruct_oreq; repeat (try etyp; casesolve)))].
 
 Local Lemma hastyp_arm_strb_reg2il:
   forall c (Xn Xm Xt extend:N) (B1:Xn < 2^5) (B2:Xm < 2^5) (B3:Xt < 2^5) (B4:extend<2^3)
@@ -4996,376 +5317,6 @@ Local Lemma hastyp_arm_ldrb_reg2il:
 Proof.
   intros; unfold_stmt. repeat econs.
 Qed.
-
-Local Lemma hastyp_arm_stxr2il_constr:
-  forall c (size Xn Xs Xt:N) (rtunknown rnunknown:exp)
-  (B1:Xn<2^5) (B2:Xs<2^5) (B3:Xt<2^5) (B4:size<=64)
-  (B6:hastyp_exp c rnunknown 64) (B7:hastyp_exp (update c (V_TEMP 1000) (Some 64)) rtunknown 64)
-  (PF:pfsub armc c),
-  hastyp_stmt armc c (arm_stxr2il_constr size Xn Xs Xt rtunknown rnunknown) armc.
-Proof.
-  intros; unfold_stmt. repeat econs; try eassumption.
-Qed.
-
-Local Lemma hastyp_arm_stxr2il_size:
-  forall c (size Xn Xs Xt:N) (rtunknown rnunknown:exp)
-  (B1:Xn<2^5) (B2:Xs<2^5) (B3:Xt<2^5) (B4:size<=64)
-  (PF:pfsub armc c),
-  hastyp_stmt armc armc (arm_stxr2il_size size Xn Xs Xt) armc.
-Proof.
-  intros; unfold_stmt. time repeat econs with hastyp_arm_stxr2il_constr.
-Qed.
-
-Local Lemma hastyp_arm_stxp2il_constr:
-  forall c (size Xn Xs Xt Xt2:N) (rtunknown rnunknown:exp)
-  (B1:Xn<2^5) (B2:Xs<2^5) (B3:Xt<2^5) (B4:size<=64) (B5:Xt2<2^5)
-  (B6:hastyp_exp empty rtunknown 1) 
-  (B7:hastyp_exp empty rnunknown 1)
-  (PF:pfsub armc c),
-  hastyp_stmt armc c (arm_stxp2il_constr size Xn Xs Xt Xt2 rtunknown rnunknown) armc.
-Proof.
-  intros; unfold_stmt. repeat econs.
-Qed.
-
-Local Lemma hastyp_arm_stxp2il_size:
-  forall c (size Xn Xs Xt Xt2:N) (rtunknown rnunknown:exp)
-  (B1:Xn<2^5) (B2:Xs<2^5) (B3:Xt<2^5) (B4:size<=64) (B5:Xt2<2^5)
-  (PF:pfsub armc c),
-  hastyp_stmt armc armc (arm_stxp2il_size size Xn Xs Xt Xt2) armc.
-Proof.
-  intros; unfold_stmt. time repeat (econs with hastyp_arm_stxp2il_constr).
-Qed.
-
-Local Lemma hastyp_arm_ldxp2il_constr:
-  forall c (size Xn Xt Xt2:N) (rtunknown:bool)
-  (B1:Xn<2^5) (B3:Xt<2^5) (B4:size=8\/size=16\/size=32\/size=64) (B5:Xt2<2^5)
-  (PF:pfsub armc c),
-  hastyp_stmt armc c (arm_ldxp2il_constr size Xn Xt Xt2 rtunknown) armc.
-Proof.
-  intros; unfold_stmt. repeat econs. all: try lia.
-Qed.
-
-Local Lemma hastyp_arm_ldxp2il_size:
-  forall c (size Xn Xt Xt2:N) (rtunknown:bool)
-  (B1:Xn<2^5) (B3:Xt<2^5) (B4:size=8\/size=16\/size=32\/size=64) (B5:Xt2<2^5)
-  (PF:pfsub armc c),
-  hastyp_stmt armc armc (arm_ldxp2il size Xn Xt Xt2) armc.
-Proof.
-  intros; unfold_stmt. time repeat (econs with hastyp_arm_ldxp2il_constr). all: try solve [simpl;lia].
-  simple_c_var.
-  subsolve; symmetry; apply typeof_arm_varid.
-  simple_c_var.
-  subsolve; symmetry; apply typeof_arm_varid.
-Qed.
-
-Local Lemma hastyp_arm_ldp2il_constr:
-  forall c Xn Xt Xt2 imm7 scale wback wb_unknown rt_unknown postindex
-  (B1:Xn<2^5) (B3:Xt<2^5) (B5:Xt2<2^5) (B6:imm7<2^7) (B7:scale=2\/scale=3)
-  (B8:forall i j k, hastyp_exp (update (update (update c (V_TEMP 1000) (Some i)) (V_TEMP 2000) (Some j)) (V_TEMP 3000) (Some k)) wback 1) 
-  (B9:forall i j k, hastyp_exp (update (update (update c (V_TEMP 1000) (Some i)) (V_TEMP 2000) (Some j)) (V_TEMP 3000) (Some k)) rt_unknown 1) 
-  (B10:forall i j k, hastyp_exp (update (update (update c (V_TEMP 1000) (Some i)) (V_TEMP 2000) (Some j)) (V_TEMP 3000) (Some k)) wb_unknown 1) 
-  (PF:pfsub armc c),
-  hastyp_stmt armc c (arm_ldp2il_constr Xn Xt Xt2 imm7 scale wback wb_unknown rt_unknown postindex) armc.
-Proof.
-  intros; unfold_stmt. repeat econs.
-  rewrite ?update_cancel; apply B9.
-  rewrite ?update_cancel. subsolve.
-  lia.
-  cget. lia.
-  eapply hastyp_exp_weaken. apply B8.  subsolve; try reflexivity. rewrite !update_frame in EQ by easy. assumption.
-  eapply hastyp_exp_weaken. apply B10. subsolve; try reflexivity. rewrite !update_frame in EQ by easy. assumption.
-  rewrite !update_cancel. subsolve. rewrite !update_frame  by (discriminate || symmetry; apply armvarid_neq_temp). reflexivity.
-  rewrite !update_cancel. subsolve. now rewrite update_updated.
-  destruct (arm_varid Xt == arm_varid Xt2) as [EQ1|NE];[rewrite EQ1|rewrite update_frame by assumption];now rewrite update_updated.
-  rewrite !update_frame by (symmetry; apply armvarid_neq_temp); now rewrite update_updated.
-  rewrite !update_frame by (discriminate||symmetry; apply armvarid_neq_temp); now rewrite update_updated.
-  rewrite !update_cancel. subsolve.
-  symmetry; c_var_reg.
-  symmetry; c_var_reg.
-Qed.
-
-(*Local Lemma hastyp_arm_ldp2il:*)
-(*  forall c Xn Xt Xt2 imm7 scale wback wb_unknown rt_unknown postindex*)
-(*  (B1:Xn<2^5) (B3:Xt<2^5) (B5:Xt2<2^5) (B6:imm7<2^7) (B7:scale=2\/scale=3)*)
-(*  (B9:forall i j k, hastyp_exp (update (update (update c (V_TEMP 1000) (Some i)) (V_TEMP 2000) (Some j)) (V_TEMP 3000) (Some k)) rt_unknown 1) *)
-(*  (B10:forall i j k, hastyp_exp (update (update (update c (V_TEMP 1000) (Some i)) (V_TEMP 2000) (Some j)) (V_TEMP 3000) (Some k)) wb_unknown 1) *)
-(*  (PF:pfsub armc c),*)
-(*  hastyp_stmt armc armc (arm_ldp2il Xn Xt Xt2 imm7 scale wback postindex) armc.*)
-(*Proof.*)
-(*  intros; unfold_stmt. repeat econs; try lia.*)
-(*  rewrite ?update_cancel. apply B9.*)
-(*  rewrite ?update_cancel. subsolve.*)
-(*  lia.*)
-(*  cget. lia.*)
-(*  eapply hastyp_exp_weaken. apply B8.  subsolve; try reflexivity. rewrite !update_frame in EQ by easy. assumption.*)
-(*  eapply hastyp_exp_weaken. apply B10. subsolve; try reflexivity. rewrite !update_frame in EQ by easy. assumption.*)
-(*  rewrite !update_cancel. subsolve. rewrite !update_frame  by (discriminate || symmetry; apply armvarid_neq_temp). reflexivity.*)
-(*  rewrite !update_cancel. subsolve. now rewrite update_updated.*)
-(*  destruct (arm_varid Xt == arm_varid Xt2) as [EQ1|NE];[rewrite EQ1|rewrite update_frame by assumption];now rewrite update_updated.*)
-(*  rewrite !update_frame by (symmetry; apply armvarid_neq_temp); now rewrite update_updated.*)
-(*  rewrite !update_frame by (discriminate||symmetry; apply armvarid_neq_temp); now rewrite update_updated.*)
-(*  rewrite !update_cancel. subsolve.*)
-(*  symmetry; c_var_reg.*)
-(*  symmetry; c_var_reg.*)
-(*Qed.*)
-
-Local Lemma hastyp_arm_ldpsw2il_constr:
-  forall c Xn Xt Xt2 imm7 wback wb_unknown rt_unknown postindex
-  (B1:Xn<2^5) (B3:Xt<2^5) (B4:imm7<2^7) (B5:Xt2<2^5)
-  (B8:forall i j k, hastyp_exp (update (update (update c (V_TEMP 1000) (Some i)) (V_TEMP 2000) (Some j)) (V_TEMP 3000) (Some k)) wback 1) 
-  (B9:forall i j k, hastyp_exp (update (update (update c (V_TEMP 1000) (Some i)) (V_TEMP 2000) (Some j)) (V_TEMP 3000) (Some k)) rt_unknown 1) 
-  (B10:forall i j k, hastyp_exp (update (update (update c (V_TEMP 1000) (Some i)) (V_TEMP 2000) (Some j)) (V_TEMP 3000) (Some k)) wb_unknown 1) 
-  (PF:pfsub armc c),
-  hastyp_stmt armc c (arm_ldpsw2il_constr Xn Xt Xt2 imm7 wback wb_unknown rt_unknown postindex) armc.
-Proof.
-  intros; unfold_stmt. repeat econs.
-  rewrite update_cancel. apply B9.
-  eapply hastyp_exp_weaken. eapply B8. subsolve; try reflexivity. rewrite !update_frame in EQ; assumption.
-  eapply hastyp_exp_weaken. eapply B10. subsolve; try reflexivity. rewrite !update_frame in EQ; assumption.
-  subsolve. symmetry; c_var_reg.
-  subsolve; symmetry; c_var_reg.
-  subsolve; symmetry; c_var_reg.
-Qed.
-
-(*Local Lemma hastyp_arm_ldpsw2il_size:*)
-(*  forall c Xn Xt Xt2 imm7 wback wb_unknown rt_unknown postindex*)
-(*  (B1:Xn<2^5) (B3:Xt<2^5) (B4:imm7<2^7) (B5:Xt2<2^5)*)
-(*  (B8:forall i j k, hastyp_exp (update (update (update c (V_TEMP 1000) (Some i)) (V_TEMP 2000) (Some j)) (V_TEMP 3000) (Some k)) wback 1) *)
-(*  (B9:forall i j k, hastyp_exp (update (update (update c (V_TEMP 1000) (Some i)) (V_TEMP 2000) (Some j)) (V_TEMP 3000) (Some k)) rt_unknown 1) *)
-(*  (B10:forall i j k, hastyp_exp (update (update (update c (V_TEMP 1000) (Some i)) (V_TEMP 2000) (Some j)) (V_TEMP 3000) (Some k)) wb_unknown 1) *)
-(*  (PF:pfsub armc c),*)
-(*  hastyp_stmt armc armc (arm_ldpsw2il_size Xn Xt Xt2 imm7 wback wb_unknown rt_unknown postindex) armc.*)
-(*Proof.*)
-(*  intros; unfold_stmt. repeat econs.*)
-(*  rewrite update_cancel. apply B9.*)
-(*  eapply hastyp_exp_weaken. eapply B8. subsolve; try reflexivity. rewrite !update_frame in EQ; assumption.*)
-(*  eapply hastyp_exp_weaken. eapply B10. subsolve; try reflexivity. rewrite !update_frame in EQ; assumption.*)
-(*  subsolve. symmetry; c_var_reg.*)
-(*  subsolve; symmetry; c_var_reg.*)
-(*  subsolve; symmetry; c_var_reg.*)
-(*Qed.*)
-
-Local Lemma hastyp_arm_strb_imm2il_constr:
-  forall c (Xn Xt imm912:N) (signed wback postindex rtunknown:bool)
-  (B1:Xn<2^5)  (B3:Xt<2^5) (B4:if signed then imm912<2^9 else imm912<2^12) 
-  (PF:pfsub armc c),
-  hastyp_stmt armc c (arm_strb_imm2il_constr Xn Xt imm912 signed wback postindex rtunknown) armc.
-Proof.
-  intros; unfold_stmt. repeat econs.
-  subsolve. simple_c_var.
-  subsolve. simple_c_var.
-Qed.
-
-(*Local Lemma hastyp_arm_strb_imm2il_size:*)
-(*  forall c (Xn Xt imm912:N) (signed wback postindex rtunknown:bool)*)
-(*  (B1:Xn<2^5)  (B3:Xt<2^5) (B4:if signed then imm912<2^9 else imm912<2^12) *)
-(*  (PF:pfsub armc c),*)
-(*  hastyp_stmt armc armc (arm_strb_imm2il_size Xn Xt imm912 signed wback postindex rtunknown) armc.*)
-(*Proof.*)
-(*  intros; unfold_stmt. repeat econs.*)
-(*  subsolve. simple_c_var.*)
-(*  subsolve. simple_c_var.*)
-(*Qed.*)
-
-Local Lemma hastyp_arm_strh_imm2il_constr:
-  forall c (Xn Xt imm912:N) (signed wback postindex rtunknown:bool)
-  (B1:Xn<2^5)  (B3:Xt<2^5) (B4:if signed then imm912<2^9 else imm912<2^12) 
-  (PF:pfsub armc c),
-  hastyp_stmt armc c (arm_strh_imm2il_constr Xn Xt imm912 signed wback postindex rtunknown) armc.
-Proof.
-  intros; unfold_stmt. repeat econs.
-  subsolve. simple_c_var.
-  subsolve. simple_c_var.
-Qed.
-
-(*Local Lemma hastyp_arm_strh_imm2il_size:*)
-(*  forall c (Xn Xt imm912:N) (signed wback postindex rtunknown:bool)*)
-(*  (B1:Xn<2^5)  (B3:Xt<2^5) (B4:if signed then imm912<2^9 else imm912<2^12) *)
-(*  (PF:pfsub armc c),*)
-(*  hastyp_stmt armc armc (arm_strh_imm2il_size Xn Xt imm912 signed wback postindex rtunknown) armc.*)
-(*Proof.*)
-(*  intros; unfold_stmt. repeat econs.*)
-(*  subsolve. simple_c_var.*)
-(*  subsolve. simple_c_var.*)
-(*Qed.*)
-
-Local Lemma hastyp_arm_str_imm2il_constr:
-  forall c (Xn Xt imm912 size:N) (signed wback postindex rtunknown:bool)
-  (B1:Xn<2^5)  (B3:Xt<2^5) (B4:if signed then imm912<2^9 else imm912<2^12) (B5:size=32\/size=64)
-  (PF:pfsub armc c),
-  hastyp_stmt armc c (arm_str_imm2il_constr Xn Xt imm912 size signed wback postindex rtunknown) armc.
-Proof.
-  intros; unfold_stmt. repeat econs.
-  subsolve. simple_c_var.
-  subsolve. simple_c_var.
-Qed.
-
-(*Local Lemma hastyp_arm_str_imm2il_size:*)
-(*  forall c (Xn Xt imm912 size:N) (signed wback postindex rtunknown:bool)*)
-(*  (B1:Xn<2^5)  (B3:Xt<2^5) (B4:if signed then imm912<2^9 else imm912<2^12) (B5:size=32\/size=64)*)
-(*  (PF:pfsub armc c),*)
-(*  hastyp_stmt armc armc (arm_str_imm2il_size Xn Xt imm912 size signed wback postindex rtunknown) armc.*)
-(*Proof.*)
-(*  intros; unfold_stmt. repeat econs.*)
-(*  subsolve. simple_c_var.*)
-(*  subsolve. simple_c_var.*)
-(*Qed.*)
-
-Local Lemma hastyp_arm_ldrb_imm2il_constr:
-  forall c (Xn Xt imm912:N) (signed wback postindex wbunknown wbsuppress:bool)
-  (B1:Xn<2^5)  (B3:Xt<2^5) (B4:if signed then imm912<2^9 else imm912<2^12) 
-  (PF:pfsub armc c),
-  hastyp_stmt armc c (arm_ldrb_imm2il_constr Xn Xt imm912 signed wback postindex wbunknown wbsuppress) armc.
-Proof.
-  intros; unfold_stmt. repeat econs.
-  subsolve; simple_c_var.
-  subsolve; simple_c_var.
-Qed.
-
-(*Local Lemma hastyp_arm_ldrb_imm2il_size:*)
-(*  forall c (Xn Xt imm912:N) (signed wback postindex wbunknown wbsuppress:bool)*)
-(*  (B1:Xn<2^5)  (B3:Xt<2^5) (B4:if signed then imm912<2^9 else imm912<2^12) *)
-(*  (PF:pfsub armc c),*)
-(*  hastyp_stmt armc armc (arm_ldrb_imm2il_size Xn Xt imm912 signed wback postindex wbunknown wbsuppress) armc.*)
-(*Proof.*)
-(*  intros; unfold_stmt. repeat econs.*)
-(*  subsolve; simple_c_var.*)
-(*  subsolve; simple_c_var.*)
-(*Qed.*)
-
-Local Lemma hastyp_arm_ldrh_imm2il_constr:
-  forall c (Xn Xt imm912:N) (signed wback postindex wbunknown wbsuppress:bool)
-  (B1:Xn<2^5)  (B3:Xt<2^5) (B4:if signed then imm912<2^9 else imm912<2^12)
-  (PF:pfsub armc c),
-  hastyp_stmt armc c (arm_ldrh_imm2il_constr Xn Xt imm912 signed wback postindex wbunknown wbsuppress) armc.
-Proof.
-  intros; unfold_stmt. repeat econs.
-  subsolve; simple_c_var.
-  subsolve; simple_c_var.
-Qed.
-
-(*Local Lemma hastyp_arm_ldrh_imm2il_size:*)
-(*  forall c (Xn Xt imm912:N) (signed wback postindex wbunknown wbsuppress:bool)*)
-(*  (B1:Xn<2^5)  (B3:Xt<2^5) (B4:if signed then imm912<2^9 else imm912<2^12)*)
-(*  (PF:pfsub armc c),*)
-(*  hastyp_stmt armc armc (arm_ldrh_imm2il_size Xn Xt imm912 signed wback postindex wbunknown wbsuppress) armc.*)
-(*Proof.*)
-(*  intros; unfold_stmt. repeat econs.*)
-(*  subsolve; simple_c_var.*)
-(*  subsolve; simple_c_var.*)
-(*Qed.*)
-
-Local Lemma hastyp_arm_ldr_imm2il_constr:
-  forall c (Xn Xt imm912 size:N) (signed wback postindex wbunknown wbsuppress:bool)
-  (B1:Xn<2^5)  (B3:Xt<2^5) (B4:if signed then imm912<2^9 else imm912<2^12) (B5:size=32\/size=64)
-  (PF:pfsub armc c),
-  hastyp_stmt armc c (arm_ldr_imm2il_constr Xn Xt imm912 size signed wback postindex wbunknown wbsuppress) armc.
-Proof.
-  intros; unfold_stmt. repeat econs. 
-  subsolve; simple_c_var.
-  subsolve; simple_c_var.
-Qed.
-
-(*Local Lemma hastyp_arm_ldr_imm2il_size:*)
-(*  forall c (Xn Xt imm912 size:N) (signed wback postindex wbunknown wbsuppress:bool)*)
-(*  (B1:Xn<2^5)  (B3:Xt<2^5) (B4:if signed then imm912<2^9 else imm912<2^12) (B5:size=32\/size=64)*)
-(*  (PF:pfsub armc c),*)
-(*  hastyp_stmt armc armc (arm_ldr_imm2il_size Xn Xt imm912 size signed wback postindex wbunknown wbsuppress) armc.*)
-(*Proof.*)
-(*  intros; unfold_stmt. repeat econs. *)
-(*  subsolve; simple_c_var.*)
-(*  subsolve; simple_c_var.*)
-(*Qed.*)
-
-Local Lemma hastyp_arm_ldrsb_imm2il_constr:
-  forall c (Xn Xt imm912 size:N) (signed wback postindex wbunknown wbsuppress:bool)
-  (B1:Xn<2^5)  (B3:Xt<2^5) (B4:if signed then imm912<2^9 else imm912<2^12) (B5:size=32\/size=64)
-  (PF:pfsub armc c),
-  hastyp_stmt armc c (arm_ldrsb_imm2il_constr Xn Xt imm912 size signed wback postindex wbunknown wbsuppress) armc.
-Proof.
-  intros; unfold_stmt. repeat econs.
-  1,3: lia.
-  subsolve; simple_c_var.
-  subsolve; simple_c_var.
-Qed.
-
-(*Local Lemma hastyp_arm_ldrsb_imm2il_size:*)
-(*  forall c (Xn Xt imm912 size:N) (signed wback postindex wbunknown wbsuppress:bool)*)
-(*  (B1:Xn<2^5)  (B3:Xt<2^5) (B4:if signed then imm912<2^9 else imm912<2^12) (B5:size=32\/size=64)*)
-(*  (PF:pfsub armc c),*)
-(*  hastyp_stmt armc armc (arm_ldrsb_imm2il_size Xn Xt imm912 size signed wback postindex wbunknown wbsuppress) armc.*)
-(*Proof.*)
-(*  intros; unfold_stmt. repeat econs.*)
-(*  1,3: lia.*)
-(*  subsolve; simple_c_var.*)
-(*  subsolve; simple_c_var.*)
-(*Qed.*)
-
-Local Lemma hastyp_arm_ldrsh_imm2il_constr:
-  forall c (Xn Xt imm912 size:N) (signed wback postindex wbunknown wbsuppress:bool)
-  (B1:Xn<2^5)  (B3:Xt<2^5) (B4:if signed then imm912<2^9 else imm912<2^12) (B4:size=32\/size=64) 
-  (PF:pfsub armc c),
-  hastyp_stmt armc c (arm_ldrsh_imm2il_constr Xn Xt imm912 size signed wback postindex wbunknown wbsuppress) armc.
-Proof.
-  intros; unfold_stmt. repeat econs.
-  1,3: lia.
-  subsolve; simple_c_var.
-  subsolve; simple_c_var.
-Qed.
-
-(*Local Lemma hastyp_arm_ldrsh_imm2il_size:*)
-(*  forall c (Xn Xt imm912 size:N) (signed wback postindex wbunknown wbsuppress:bool)*)
-(*  (B1:Xn<2^5)  (B3:Xt<2^5) (B4:if signed then imm912<2^9 else imm912<2^12) (B4:size=32\/size=64) *)
-(*  (PF:pfsub armc c),*)
-(*  hastyp_stmt armc armc (arm_ldrsh_imm2il_size Xn Xt imm912 size signed wback postindex wbunknown wbsuppress) armc.*)
-(*Proof.*)
-(*  intros; unfold_stmt. repeat econs.*)
-(*  1,3: lia.*)
-(*  subsolve; simple_c_var.*)
-(*  subsolve; simple_c_var.*)
-(*Qed.*)
-
-Local Lemma hastyp_arm_ldrsw_imm2il_constr:
-  forall c (Xn Xt imm912:N) (signed wback postindex wbunknown wbsuppress:bool)
-  (B1:Xn<2^5)  (B3:Xt<2^5) (B4:if signed then imm912<2^9 else imm912<2^12)  
-  (PF:pfsub armc c),
-  hastyp_stmt armc c (arm_ldrsw_imm2il_constr Xn Xt imm912 signed wback postindex wbunknown wbsuppress) armc.
-Proof.
-  intros; unfold_stmt. repeat econs.
-  subsolve; simple_c_var.
-  subsolve; simple_c_var.
-Qed.
-
-(*Local Lemma hastyp_arm_ldrsw_imm2il_size:*)
-(*  forall c (Xn Xt imm912:N) (signed wback postindex wbunknown wbsuppress:bool)*)
-(*  (B1:Xn<2^5)  (B3:Xt<2^5) (B4:if signed then imm912<2^9 else imm912<2^12)  *)
-(*  (PF:pfsub armc c),*)
-(*  hastyp_stmt armc armc (arm_ldrsw_imm2il_size Xn Xt imm912 signed wback postindex wbunknown wbsuppress) armc.*)
-(*Proof.*)
-(*  intros; unfold_stmt. repeat econs.*)
-(*  subsolve; simple_c_var.*)
-(*  subsolve; simple_c_var.*)
-(*Qed.*)
-
-Local Lemma hastyp_arm_ldraa2il_constr:
-  forall c (Xn Xt S imm9:N) (wback wbunknown wbsuppress:bool)
-  (B1:Xn<2^5)  (B3:Xt<2^5) (B4:S<2^1) (B5:imm9<2^9) 
-  (PF:pfsub armc c),
-  hastyp_stmt armc c (arm_ldraa2il_constr Xn Xt S imm9 wback wbunknown wbsuppress) armc.
-Proof.
-  intros; unfold_stmt. repeat econs.
-  subsolve. simple_c_var. 
-Qed.
-
-(*Local Lemma hastyp_arm_ldraa2il_size:*)
-(*  forall c (Xn Xt S imm9:N) (wback wbunknown wbsuppress:bool)*)
-(*  (B1:Xn<2^5)  (B3:Xt<2^5) (B4:S<2^1) (B5:imm9<2^9) *)
-(*  (PF:pfsub armc c),*)
-(*  hastyp_stmt armc armc (arm_ldraa2il_size Xn Xt S imm9 wback wbunknown wbsuppress) armc.*)
-(*Proof.*)
-(*  intros; unfold_stmt. repeat econs.*)
-(*  subsolve. simple_c_var. *)
-(*Qed.*)
 
 Local Lemma hastyp_arm_ldrsb_reg2il:
   forall c Xn Xm Xt size extend (B1:Xn<2^5) (B2:Xm<2^5) (B3:Xt<2^5) (B4:extend<2^3) (B5:size=32\/size=64) (PF:pfsub armc c),
@@ -5555,6 +5506,7 @@ Proof.
   intros; unfold_stmt. repeat econs. casesolve.
   all: etyp; try (rewrite update_updated; reflexivity).
   1-14: try apply hastyp_exp_weaken with (c1:=c); try eassumption; try subsolve.
+  rewrite N.mul_comm; econs.
 Qed.
 
 Local Lemma hastyp_arm_ldatomic2il_size:
@@ -5568,6 +5520,8 @@ Proof.
   subsolve.
   1-2:c_varx.
   repeat econs.
+  subsolve.
+  symmetry. apply PF, typeof_arm_varid.
 Qed.
 
 Local Lemma hastyp_arm_swp2il_size:
@@ -5807,27 +5761,107 @@ Proof.
   repeat (destruct p; try discriminate).
 Qed.
 
-Local Lemma hastyp_arm_log_imm2il:
-  forall op Rn Rd immr imms sf n_ q,
+Ltac sub_prover:=
+intros x y X; rewrite ?update_frame by (intro; subst; discriminate);try assumption.
+
+Local Lemma hastyp_arm_log_imm:
+  forall op Rn Rd immr imms sf n_,
    (n_ < 2)->(sf = 1\/ sf =0)->(imms < 2^6) -> (immr < 2^6)-> (Rn < 2^5) -> (Rd < 2 ^ 5) ->
-   arm_log_imm2il op Rn Rd immr imms sf n_ = Some q ->
-    hastyp_stmt armc armc q armc.
+    hastyp_stmt armc armc (arm_log_imm2il op Rn Rd immr imms sf n_) armc.
 Proof.
-  intros. unfold arm_log_imm2il in *. destruct op; match type of H5 with ?l = _ => revert H5; unfold_rec l end.
-  all: destruct_match_rmr.
-  all: try discriminate.
-  all: intros H5; try destruct_match_in H5; try discriminate; inversion H5; try subst q; clear H5.
-  all: try rewrite N.eqb_eq in *; try subst sf.
-  all: try solve [repeat econs; solve_armc_sub || lia].
-  - repeat econs; lia || solve_armc_sub || idtac. etyp'; try repeat casesolve.
-      apply lnot_bound, wmask_bound; lia.
-  - repeat econs; lia || solve_armc_sub || idtac. etyp'; try repeat casesolve.
-      apply lnot_bound, wmask_bound; lia.
-  - repeat econs; lia || solve_armc_sub || idtac. etyp'; try repeat casesolve.
-  - repeat econs; lia || solve_armc_sub || idtac. etyp'; try repeat casesolve.
-  - repeat econs; lia || solve_armc_sub || idtac. etyp'; try repeat casesolve.
-  - repeat econs; lia || solve_armc_sub || idtac. etyp'; try repeat casesolve.
-Qed.
+  intros. unfold_stmt.
+  destruct op eqn:?.   
+  - unfold_stmt. estyp; try assumption; try reflexivity. lia. 
+  eapply hastyp_DecodeBitMasks. 1-3: assumption. lia.
+  destruct (sf =?1); lia.
+  eapply hastyp_XtoVar. destruct (sf =?1). 
+  sub_prover. sub_prover. 
+  assumption. destruct (sf =?1); lia.
+  unfold sizeof_c. 
+  eapply typeof_arm_varid. reflexivity.
+  unfold widthof_binop, sizeof_c. rewrite update_updated. destruct (sf =?1); lia.
+  apply update_sub. repeat rewrite update_frame. apply typeof_arm_varid. 
+  all: try eapply varid_neq_temp.
+  sub_prover.
+
+  - unfold_stmt. destruct H0 as [|]; subst; psimpl.  
+  -- estyp; try assumption; try reflexivity. 
+  eapply hastyp_DecodeBitMasks. 1-3: assumption. lia. lia.
+  eapply hastyp_XtoVar. 
+  sub_prover. assumption. apply typeof_arm_varid.
+   unfold sizeof_c. rewrite update_updated. 
+  rewrite update_swap with (x1:=temp[980])(x2:=temp[1000]) by congruence.
+  apply update_updated. 
+  apply update_sub. repeat rewrite update_frame. apply typeof_arm_varid. 
+  all: try eapply varid_neq_temp. eapply hastyp_XtoVar. sub_prover. assumption.
+  eapply update_some. repeat rewrite update_frame by discriminate. reflexivity.
+  reflexivity.
+  eapply hastyp_XtoVar. sub_prover. assumption. 
+  eapply update_some. repeat rewrite update_frame by discriminate. reflexivity.
+  reflexivity.
+  eapply update_some. repeat rewrite update_frame by discriminate. reflexivity.
+  reflexivity.
+  eapply update_some. repeat rewrite update_frame by discriminate. reflexivity.
+  reflexivity.
+  sub_prover. 
+
+    -- estyp; try assumption; try reflexivity. 
+  eapply hastyp_DecodeBitMasks. 1-3: assumption. lia. lia.
+  eapply hastyp_XtoVar. 
+  sub_prover. assumption. apply typeof_arm_varid.
+   unfold sizeof_c. rewrite update_updated. 
+  rewrite update_swap with (x1:=temp[980])(x2:=temp[1000]) by congruence.
+  apply update_updated. 
+  unfold widthof_binop, sizeof_c.
+  rewrite update_updated. lia.
+  apply update_sub. repeat rewrite update_frame. apply typeof_arm_varid. 
+  all: try eapply varid_neq_temp. eapply hastyp_XtoVar. sub_prover. assumption.
+  eapply update_some. repeat rewrite update_frame by discriminate. reflexivity.
+  reflexivity.
+  eapply hastyp_XtoVar. sub_prover. assumption. 
+  eapply update_some. repeat rewrite update_frame by discriminate. reflexivity.
+  reflexivity.
+  eapply update_some. repeat rewrite update_frame by discriminate. reflexivity.
+  reflexivity.
+  eapply update_some. repeat rewrite update_frame by discriminate. reflexivity.
+  reflexivity.
+  sub_prover.
+  
+
+   - unfold_stmt. estyp; try assumption; try reflexivity. lia. 
+  eapply hastyp_DecodeBitMasks. 1-3: assumption. lia.
+  destruct (sf =?1); lia.
+  eapply hastyp_XtoVar. destruct (sf =?1). 
+  sub_prover. sub_prover. 
+  assumption. destruct (sf =?1); lia.
+  unfold sizeof_c. 
+  eapply typeof_arm_varid. reflexivity.
+  unfold widthof_binop, sizeof_c. rewrite update_updated. destruct (sf =?1); lia.
+  apply update_sub. repeat rewrite update_frame. apply typeof_arm_varid. 
+  all: try eapply varid_neq_temp.
+  sub_prover.
+  
+  - unfold_stmt. estyp; try assumption; try reflexivity. lia. 
+  eapply hastyp_DecodeBitMasks. 1-3: assumption. lia.
+  destruct (sf =?1); lia.
+  eapply hastyp_XtoVar. destruct (sf =?1). 
+  sub_prover. sub_prover. 
+  assumption. destruct (sf =?1); lia.
+  unfold sizeof_c. 
+  eapply typeof_arm_varid. reflexivity.
+  unfold widthof_binop, sizeof_c. rewrite update_updated. destruct (sf =?1); lia.
+  apply update_sub. repeat rewrite update_frame. apply typeof_arm_varid. 
+  all: try eapply varid_neq_temp.
+  sub_prover.
+
+  (*arm_bfm_imm2il*)
+  - unfold_stmt. repeat econs. etyp; try assumption; try lia.  
+  lia. lia.
+  rewrite <- store_upd_eq. sub_prover. repeat rewrite update_frame by eapply varid_neq_temp.
+  eapply typeof_arm_varid. lia. lia.
+  rewrite <- store_upd_eq. sub_prover. repeat rewrite update_frame by eapply varid_neq_temp.
+  eapply typeof_arm_varid. 
+Admitted.
 
 Local Lemma hastyp_arm_mov_imm:
   forall op Rd imm16 size shift,
@@ -5836,204 +5870,13 @@ Proof.
 Admitted.
 
 
-  (*final arm2il-C6.2.5*)
-  Definition arm2il (a:addr) inst:=
-  let il := match inst with
-  (*DP imm*)
-  | ARM_DATA_IMM op sf s sh imm12 Rn Rd => arm_data_imm2il op sf s sh imm12 Rn Rd
-  (*logical imm*)
-  | ARM_LOGICAL_IMM op Rn Rd immr imms sf n_ => arm_log_imm2il op Rn Rd immr imms sf n_
-  (*move wide*)
-  | ARM_MOVE_IMM op Rd imm16 size shift => arm_mov_imm2il op Rd imm16 size shift
-  (*PC relative addressing*)
-(*| ARM_ADRP_IMM
-  | ARM_ADR_IMM *)
-  (*compare immediate*)
-  | ARM_CCMN_IMM sf Rn imm nzcv cond => arm_data_i_with_cond (ARM_CCMN_IMM sf Rn imm nzcv cond) sf Rn imm nzcv cond
-  | ARM_CCMP_IMM sf Rn imm nzcv cond => arm_data_i_with_cond (ARM_CCMP_IMM sf Rn imm nzcv cond) sf Rn imm nzcv cond
-  (*DP reg*)
-  (*arith extended*)
-  | ARM_EXTENDED op sf s opt Rm option_ imm3 Rn Rd => arm_extend_reg2il op 0 sf s Rm option_ imm3 Rn Rd
-  (*arith shifted*)
-  | ARM_DATA_SHIFTED op sf s shift Rm imm6 Rn Rd => arm_datashft_reg2il op 0 sf s shift Rm Rd imm6 Rn
-  (*logical shifted*)
-  | ARM_LOG_SHIFTED op sf shift Rm imm6 Rn Rd => arm_logshft_reg2il op 0 sf 0 shift Rm Rd imm6 Rn
-  (*carry operations*)
-  | ARM_CARRY op sf s Rm Rn Rd=> arm_withcarry_2il op sf Rm Rn Rd
-  (*shift register*)
-  | ARM_SHIFT _ sf Rm op2 Rn Rd => arm_data_r_shift_il sf Rm op2 Rn Rd true false
-  (*conditional comparison*)
-  | ARM_CCMN_REG sf Rm cond Rn nzcv=> arm_data_r_with_cond ARM_CCMN_REG_V cond sf Rm Rn nzcv
-  | ARM_CCMP_REG sf Rm cond Rn nzcv=> arm_data_r_with_cond ARM_CCMP_REG_V cond sf Rm Rn nzcv
-  (*rev*)
-  | ARM_BITOPS op sf Rn Rd => arm_data_rev_il op sf Rd
-  (*branch*)
-  | ARM_B_COND cond imm19 => arm_b_cond2il cond imm19
-  (*unconditional branch(register)*)
-  | ARM_BR Xn => arm_br2il Xn
-  | ARM_BLR Xn => arm_blr2il Xn
-  | ARM_RET Xn => arm_ret2il Xn
-  (*unconditional branch(imm)*)
-  | ARM_B imm26 => arm_b2il imm26
-  | ARM_BL imm26 => arm_bl2il imm26
-  (*compare and branch(imm)*)
-  | ARM_CBZ Rt imm19 size => arm_cbz2il Rt imm19 size
-  | ARM_CBNZ Rt imm19 size => arm_cbnz2il Rt imm19 size
-  (*test and branch(imm)*)
-  | ARM_TBZ Rt imm14 b5 b40 => arm_tbz2il Rt imm14 b5 b40
-  | ARM_TBNZ Rt imm14 b5 b40 => arm_tbnz2il Rt imm14 b5 b40
-(*Loads and Stores*)
-  (*exclusive/others*)
-  | ARM_EXCLUSIVE ARM_STXRB size Xn Xs Xt Xt2 => arm_stxrb2il Xn Xs Xt
-  | ARM_EXCLUSIVE ARM_STLXRB size Xn Xs Xt Xt2 => arm_stlxrb2il Xn Xs Xt
-  | ARM_EXCLUSIVE ARM_LDXRB size Xn Xs Xt Xt2 => arm_ldxrb2il Xn Xt
-  | ARM_EXCLUSIVE ARM_LDXRH size Xn Xs Xt Xt2 => arm_ldxrh2il Xn Xt
-  | ARM_EXCLUSIVE ARM_LDAXRH size Xn Xs Xt Xt2 => arm_ldaxrh2il Xn Xt
-  | ARM_EXCLUSIVE ARM_LDAXRB size Xn Xs Xt Xt2 => arm_ldaxrb2il Xn Xt
-  | ARM_EXCLUSIVE ARM_STLLRB size Xn Xs Xt Xt2 => arm_stllrb2il Xn Xt
-  | ARM_EXCLUSIVE ARM_STLLRH size Xn Xs Xt Xt2 => arm_stllrh2il Xn Xt
-  | ARM_EXCLUSIVE ARM_STLRH size Xn Xs Xt Xt2 => arm_stlrh2il Xn Xt
-  | ARM_EXCLUSIVE ARM_STLRB size Xn Xs Xt Xt2 => arm_stlrb2il Xn Xt
-  | ARM_EXCLUSIVE ARM_STXRH size Xn Xs Xt Xt2 => arm_stxrh2il Xn Xs Xt
-  | ARM_EXCLUSIVE ARM_STLXRH size Xn Xs Xt Xt2 => arm_stlxrh2il Xn Xs Xt
-  | ARM_EXCLUSIVE ARM_LDLARB size Xn Xs Xt Xt2 => arm_ldlarb2il Xn Xt
-  | ARM_EXCLUSIVE ARM_LDARB size Xn Xs Xt Xt2 => arm_ldarb2il Xn Xt
-  | ARM_EXCLUSIVE ARM_LDARH size Xn Xs Xt Xt2 => arm_ldarh2il Xn Xt
-  | ARM_EXCLUSIVE ARM_LDLARH size Xn Xs Xt Xt2 => arm_ldlarh2il Xn Xt
-  | ARM_EXCLUSIVE ARM_STXR size Xn Xs Xt Xt2 => arm_stxr2il size Xn Xs Xt
-  | ARM_EXCLUSIVE ARM_STLXR size Xn Xs Xt Xt2 => arm_stxr2il_size size Xn Xs Xt
-  | ARM_EXCLUSIVE ARM_STXP size Xn Xs Xt Xt2 => arm_stxp2il size Xn Xs Xt Xt2
-  | ARM_EXCLUSIVE ARM_STLXP size Xn Xs Xt Xt2 => arm_stlxp2il size Xn Xs Xt Xt2
-  | ARM_EXCLUSIVE ARM_LDXR size Xn Xs Xt Xt2 => arm_ldxr2il size Xn Xt
-  | ARM_EXCLUSIVE ARM_LDAXR size Xn Xs Xt Xt2 => arm_ldaxr2il size Xn Xt
-  | ARM_EXCLUSIVE ARM_LDXP size Xn Xs Xt Xt2 => arm_ldxp2il size Xn Xt Xt2
-  | ARM_EXCLUSIVE ARM_LDAXP size Xn Xs Xt Xt2 => havoc
-  | ARM_EXCLUSIVE ARM_STLLR size Xn Xs Xt Xt2 => arm_stllr2il size Xn Xt
-  | ARM_EXCLUSIVE ARM_STLR size Xn Xs Xt Xt2 => arm_stlr2il size Xn Xt
-  | ARM_EXCLUSIVE ARM_LDLAR size Xn Xs Xt Xt2 => arm_ldlar2il size Xn Xt
-  | ARM_EXCLUSIVE ARM_LDAR size Xn Xs Xt Xt2 => arm_ldar2il size Xn Xt
-  (*bunch of variants for these, refer to page C4-230*)
-  | ARM_EXCLUSIVE ARM_CASP size Xn Xs Xt Xt2 => arm_casp2il Xn Xs Xt size
-  | ARM_EXCLUSIVE ARM_CASB size Xn Xs Xt Xt2 => arm_casb2il Xn Xs Xt
-  | ARM_EXCLUSIVE ARM_CASH size Xn Xs Xt Xt2 => arm_cash2il Xn Xs Xt
-  | ARM_EXCLUSIVE ARM_CAS size Xn Xs Xt Xt2 => arm_cas2il Xn Xs Xt size
-  (*LDAPR/STLR unscaled immediate*)
-  | ARM_LOAD_GEN ARM_STLURB Xn Xt imm9 size => arm_stlurb2il Xn Xt imm9
-  | ARM_LOAD_GEN ARM_LDAPURB Xn Xt imm9 size => arm_ldapurb2il Xn Xt (Word imm9 64)
-  | ARM_LOAD_GEN ARM_LDAPURSB Xn Xt imm9 size => arm_ldapursb2il Xn Xt (Word imm9 64) size
-  | ARM_LOAD_GEN ARM_STLURH Xn Xt imm9 size => arm_stlurh2il Xn Xt (Word imm9 64)
-  | ARM_LOAD_GEN ARM_LDAPURH Xn Xt imm9 size => arm_ldapurh2il Xn Xt (Word imm9 64)
-  | ARM_LOAD_GEN ARM_LDAPURSH Xn Xt imm9 size => arm_ldapursh2il Xn Xt (Word imm9 64) size
-  | ARM_LOAD_GEN ARM_LDAPUR Xn Xt imm9 size => arm_ldapur2il Xn Xt (Word imm9 64) size
-  | ARM_LOAD_GEN ARM_LDAPURSW Xn Xt imm9 size => arm_ldapursw2il Xn Xt (Word imm9 64) size
-  | ARM_LOAD_GEN ARM_STLUR Xn Xt imm9 size => arm_stlur2il Xn Xt (Word imm9 64) size
-  | ARM_LOAD_GEN ARM_PRFM Xn Xt imm9 size => arm_prfm_lit2il Xt imm9
-  | ARM_LOAD_GEN ARM_PRFM_IMM Xn Xt imm9 size => havoc
-  | ARM_ATOMIC ARM_LDAPRB size Xn Xs Xt => arm_ldaprb2il Xn Xt
-  | ARM_ATOMIC ARM_LDAPRH size Xn Xs Xt => arm_ldaprh2il Xn Xt
-  | ARM_ATOMIC ARM_LDAPR size Xn Xs Xt => arm_ldapr2il size Xn Xt
-  (*load/store memory tags*)
-  | ARM_STG Xn Xt imm9 writeback printindex => arm_stg2il Xn Xt imm9 writeback printindex
-  | ARM_STZG Xn Xt imm9 writeback printindex => arm_stzg2il Xn Xt imm9 writeback printindex
-  | ARM_STZGM Xn Xt => arm_stzgm2il Xt Xn
-  | ARM_LDG Xn Xt imm9 => arm_ldg2il Xn Xt imm9
-  | ARM_ST2G Xn Xt imm9 writeback printindex => arm_st2g2il Xn Xt imm9 writeback printindex
-  | ARM_STGM Xn Xt => arm_stgm2il Xn Xt
-  | ARM_STZ2G Xn Xt imm9 writeback printindex => arm_stz2g2il Xn Xt imm9 writeback printindex
-  | ARM_LDGM Xn Xt => arm_ldgm2il Xn Xt
-  (*load register (literal)*)
-  | ARM_LD_REG_LIT ARM_LDR_LIT Xt imm19 size => arm_ldr_lit2il Xt imm19 size
-  | ARM_LD_REG_LIT ARM_LDRSW_LIT Xt imm19 size => arm_ldrsw_lit2il Xt imm19
-  | ARM_LD_REG_LIT ARM_PRFM_LIT Xt imm19 size => arm_prfm_lit2il Xt imm19
-  (*load/store no-allocate pair (offset)*)
-  | ARM_STNP Xn Xt Xt2 imm7 scale => arm_stnp2il Xn Xt Xt2 imm7 scale
-  | ARM_LDNP Xn Xt Xt2 imm7 scale => arm_stnp2il Xn Xt Xt2 imm7 scale
-  (*load/store register pair (post-indexed, pre-indexed, offset)*)
-  | ARM_LD_STR_REG_PAIR ARM_STP Xn Xt Xt2 imm7 scale wback postindex => arm_stp2il Xn Xt Xt2 imm7 scale wback postindex
-  | ARM_LD_STR_REG_PAIR ARM_LDP Xn Xt Xt2 imm7 scale wback postindex => arm_ldp2il Xn Xt Xt2 imm7 scale wback postindex
-  | ARM_LD_STR_REG_PAIR ARM_LDPSW Xn Xt Xt2 imm7 scale wback postindex => arm_ldpsw2il Xn Xt Xt2 imm7 wback postindex
-  | ARM_LD_STR_REG_PAIR ARM_STGP Xn Xt Xt2 imm7 scale wback postindex => arm_stgp2il Xn Xt Xt2 imm7 wback postindex
-  (*load/store register (unscaled immediate)*)
-  | ARM_LOAD_GEN ARM_STURB Xn Xt imm9 _ => arm_sturb2il Xn Xt imm9
-  | ARM_LOAD_GEN ARM_LDURB Xn Xt imm9 _ => arm_ldurb2il Xn Xt imm9
-  | ARM_LOAD_GEN ARM_LDURSB Xn Xt imm9 size => arm_ldursb2il Xn Xt imm9 size
-  | ARM_LOAD_GEN ARM_STURH Xn Xt imm9 _ => arm_sturh2il Xn Xt imm9
-  | ARM_LOAD_GEN ARM_LDURH Xn Xt imm9 _ => arm_ldurh2il Xn Xt imm9
-  | ARM_LOAD_GEN ARM_LDURSH Xn Xt imm9 size => arm_ldursh2il Xn Xt imm9 size
-  | ARM_LOAD_GEN ARM_STUR Xn Xt imm9 size => arm_stur2il Xn Xt imm9 size
-  | ARM_LOAD_GEN ARM_LDUR Xn Xt imm9 size => arm_ldur2il Xn Xt imm9 size
-  | ARM_LOAD_GEN ARM_LDURSW Xn Xt imm9 _ => arm_ldursw2il Xn Xt imm9
-  (*imm pre/post-indexed*)
-  | ARM_INDEXED ARM_STRB_IMM Xn Xt imm912 size signed wback postindex => arm_strb_imm2il Xn Xt imm912 signed wback postindex
-  | ARM_INDEXED ARM_LDRB_IMM Xn Xt imm912 size signed wback postindex => arm_ldrb_imm2il Xn Xt imm912 signed wback postindex
-  | ARM_INDEXED ARM_LDRSB_IMM Xn Xt imm912 size signed wback postindex => arm_ldrsb_imm2il Xn Xt imm912 size signed wback postindex
-  | ARM_INDEXED ARM_LDR_IMM Xn Xt imm912 size signed wback postindex => arm_ldr_imm2il Xn Xt imm912 size signed wback postindex
-  | ARM_INDEXED ARM_STRH_IMM Xn Xt imm912 size signed wback postindex => arm_strh_imm2il Xn Xt imm912 size signed wback postindex (*TODO: whats size?*)
-  | ARM_INDEXED ARM_LDRH_IMM Xn Xt imm912 size signed wback postindex => arm_ldrh_imm2il Xn Xt imm912 signed wback postindex
-  | ARM_INDEXED ARM_LDRSH_IMM Xn Xt imm912 size signed wback postindex => arm_ldrsh_imm2il Xn Xt imm912 size signed wback postindex
-  | ARM_INDEXED ARM_STR_IMM Xn Xt imm912 size signed wback postindex => arm_str_imm2il Xn Xt imm912 size signed wback postindex
-  | ARM_INDEXED ARM_LDRSW_IMM Xn Xt imm912 size signed wback postindex => arm_ldrsw_imm2il Xn Xt imm912 signed wback postindex
-  (*register unprivileged*)
-  | ARM_REG_UNPRIVILEGED ARM_STTRB Rn Rt imm9 size => arm_sttrb2il Rn Rt imm9
-  | ARM_REG_UNPRIVILEGED ARM_LDTRB Rn Rt imm9 size => arm_ldtrb2il Rn Rt imm9
-  | ARM_REG_UNPRIVILEGED ARM_LDTRSB Rn Rt imm9 size => arm_ldtrsb2il Rn Rt imm9 size
-  | ARM_REG_UNPRIVILEGED ARM_STTRH Rn Rt imm9 size => arm_sttrh2il Rn Rt imm9
-  | ARM_REG_UNPRIVILEGED ARM_LDTRH Rn Rt imm9 size => arm_ldtrh2il Rn Rt imm9
-  | ARM_REG_UNPRIVILEGED ARM_LDTRSH Rn Rt imm9 size => arm_ldtrsh2il Rn Rt imm9 size
-  | ARM_REG_UNPRIVILEGED ARM_STTR Rn Rt imm9 size => arm_sttr2il Rn Rt imm9 size
-  | ARM_REG_UNPRIVILEGED ARM_LDTR Rn Rt imm9 size => arm_ldtr2il Rn Rt imm9 size
-  | ARM_REG_UNPRIVILEGED ARM_LDTRSW Rn Rt imm9 size => arm_ldtrsw2il Rn Rt imm9
-  (*atomic memory ops*)
-  | ARM_ATOMIC ARM_LDADDB size Xn Xs Xt => arm_ldaddb2il Xn Xs Xt
-  | ARM_ATOMIC ARM_LDCLRB size Xn Xs Xt => arm_ldclrb2il Xn Xs Xt
-  | ARM_ATOMIC ARM_LDEORB size Xn Xs Xt => arm_ldeorb2il Xn Xs Xt
-  | ARM_ATOMIC ARM_LDSETB size Xn Xs Xt => arm_ldsetb2il Xn Xs Xt
-  | ARM_ATOMIC ARM_LDSMAXB size Xn Xs Xt => arm_ldsmaxb2il Xn Xs Xt
-  | ARM_ATOMIC ARM_LDSMINB size Xn Xs Xt => arm_ldsminb2il Xn Xs Xt
-  | ARM_ATOMIC ARM_LDUMINB size Xn Xs Xt => arm_lduminb2il Xn Xs Xt
-  | ARM_ATOMIC ARM_SWPB size Xn Xs Xt => arm_swpb2il Xn Xs Xt
-  | ARM_ATOMIC ARM_LDADDH size Xn Xs Xt => arm_ldaddh2il Xn Xs Xt
-  | ARM_ATOMIC ARM_LDCLRH size Xn Xs Xt => arm_ldclrh2il Xn Xs Xt
-  | ARM_ATOMIC ARM_LDEORH size Xn Xs Xt => arm_ldeorh2il Xn Xs Xt
-  | ARM_ATOMIC ARM_LDSETH size Xn Xs Xt => arm_ldseth2il Xn Xs Xt
-  | ARM_ATOMIC ARM_LDSMAXH size Xn Xs Xt => arm_ldsmaxh2il Xn Xs Xt
-  | ARM_ATOMIC ARM_LDSMINH size Xn Xs Xt => arm_ldsminh2il Xn Xs Xt
-  | ARM_ATOMIC ARM_LDUMAXH size Xn Xs Xt => arm_ldumaxh2il Xn Xs Xt
-  | ARM_ATOMIC ARM_LDUMINH size Xn Xs Xt => arm_lduminh2il Xn Xs Xt
-  | ARM_ATOMIC ARM_SWPH size Xn Xs Xt => arm_swph2il Xn Xs Xt
-  | ARM_ATOMIC ARM_LDADD size Xn Xs Xt => arm_ldadd2il size Xn Xs Xt
-  | ARM_ATOMIC ARM_LDCLR size Xn Xs Xt => arm_ldclr2il size Xn Xs Xt
-  | ARM_ATOMIC ARM_LDEOR size Xn Xs Xt => arm_ldeor2il size Xn Xs Xt
-  | ARM_ATOMIC ARM_LDSET size Xn Xs Xt => arm_ldset2il size Xn Xs Xt
-  | ARM_ATOMIC ARM_LDSMAX size Xn Xs Xt => arm_ldsmax2il size Xn Xs Xt
-  | ARM_ATOMIC ARM_LDSMIN size Xn Xs Xt => arm_ldsmin2il size Xn Xs Xt
-  | ARM_ATOMIC ARM_LDUMAX size Xn Xs Xt => arm_ldumax2il size Xn Xs Xt
-  | ARM_ATOMIC ARM_LDUMIN size Xn Xs Xt => arm_ldumin2il size Xn Xs Xt
-  | ARM_ATOMIC ARM_SWP size Xn Xs Xt => arm_swp2il size Xn Xs Xt
-  (*there's a lot more here, not sure how much to add. Pages C4-240-250*)
-  (*pac*)
-  | ARM_LDRAA Xn Xt s imm9 wback => arm_ldraa2il Xn Xt s imm9 wback
-  (*load/store register*)
-  | ARM_LD_STR_REG ARM_STRB_REG Xn Xm Xt extend _ _ => arm_strb_reg2il Xn Xm Xt extend
-  | ARM_LD_STR_REG ARM_LDRB_REG Xn Xm Xt extend _ _ => arm_ldrb_reg2il Xn Xm Xt extend
-  | ARM_LD_STR_REG ARM_LDRSB_REG Xn Xm Xt extend size _=> arm_ldrsb_reg2il Xn Xm Xt size extend
-  | ARM_LD_STR_REG ARM_STRH_REG Xn Xm Xt extend _ s => arm_strh_reg2il Xn Xm Xt extend s
-  | ARM_LD_STR_REG ARM_LDRH_REG Xn Xm Xt extend _ s => arm_ldrh_reg2il Xn Xm Xt extend s
-  | ARM_LD_STR_REG ARM_LDRSH_REG Xn Xm Xt extend size s => arm_ldrsh_reg2il Xn Xm Xt extend size s
-  | ARM_LD_STR_REG ARM_STR_REG Xn Xm Xt extend size s => arm_str_reg2il Xn Xm Xt extend size s
-  | ARM_LD_STR_REG ARM_LDR_REG Xn Xm Xt extend size s => arm_ldr_reg2il Xn Xm Xt extend size s
-  | ARM_LD_STR_REG ARM_LDRSW_REG Xn Xm Xt extend _ s => arm_ldrsw_reg2il Xn Xm Xt extend s
- (* | ARM_LD_STR_REG ARM_PRFM_REG Xn Xm Xt extend _ s => havoc*)
-  | UDF => Exn 4
-  |_ => havoc end in
-  Seq (Move R_PC (Word (a mod 2^64) 64)) il.
-End Decoder.
-
 Theorem welltyped_arm82il:
   forall a n, hastyp_stmt armc armc (arm2il a (arm_decode n)) arm8typctx.
 Proof.
   intros. unfold_stmt. styp. now apply N.mod_lt.
-  remember (arm_decode n) as i.
+  remember (arm_decode n) as i. 
   destruct i. apply hastyp_arm_data_imm. admit.
-Admitted.
+Admitted. 
+
+
 
